theories/channel/proto.v
@@ -24,7 +24,6 @@ notions, such as contractiveness and non-expansiveness, after which the
 specifications of the message-passing primitives are defined in terms of the
 protocol connectives. *)
 From iris.algebra Require Import excl_auth.
-From iris.bi Require Import telescopes.
 From iris.proofmode Require Import tactics.
 From iris.base_logic Require Export lib.iprop.
 From iris.base_logic Require Import lib.own.
@@ -48,6 +47,81 @@ Proof. solve_inG. Qed.
 Definition iProto Σ V := proto V (iPropO Σ) (iPropO Σ).
 Delimit Scope proto_scope with proto.
 Bind Scope proto_scope with iProto.
+Local Open Scope proto.
+
+(** * Messages *)
+Section iMsg.
+  Set Primitive Projections.
+  Record iMsg Σ V := IMsg { iMsg_car :> V → laterO (iProto Σ V) -n> iPropO Σ }.
+End iMsg.
+Arguments IMsg {_ _} _.
+Arguments iMsg_car {_ _} _.
+
+Delimit Scope msg_scope with msg.
+Bind Scope msg_scope with iMsg.
+Instance iMsg_inhabited {Σ V} : Inhabited (iMsg Σ V) := populate (IMsg inhabitant).
+
+Section imsg_ofe.
+  Context {Σ : gFunctors} {V : Type}.
+
+  Instance iMsg_equiv : Equiv (iMsg Σ V) := λ m1 m2,
+    ∀ w p, iMsg_car m1 w p ≡ iMsg_car m2 w p.
+  Instance iMsg_dist : Dist (iMsg Σ V) := λ n m1 m2,
+    ∀ w p, iMsg_car m1 w p ≡{n}≡ iMsg_car m2 w p.
+
+  Lemma iMsg_ofe_mixin : OfeMixin (iMsg Σ V).
+  Proof. by apply (iso_ofe_mixin (iMsg_car : _ → V -d> _ -n> _)). Qed.
+  Canonical Structure iMsgO := OfeT (iMsg Σ V) iMsg_ofe_mixin.
+
+  Global Instance iMsg_cofe : Cofe iMsgO.
+  Proof. by apply (iso_cofe (IMsg : (V -d> _ -n> _) → _) iMsg_car). Qed.
+
+  Global Instance iMsg_car_ne n : Proper (dist n ==> (=) ==> dist n) iMsg_car.
+  Proof. by intros m m' ? w ? <- p. Qed.
+  Global Instance iMsg_car_proper : Proper ((≡) ==> (=) ==> (≡)) iMsg_car.
+  Proof. by intros m m' ? w ? <- p. Qed.
+
+  Global Instance IMsg_ne n : Proper (pointwise_relation _ (dist n) ==> dist n) IMsg.
+  Proof. by intros ???. Qed.
+  Global Instance IMsg_proper : Proper (pointwise_relation _ (≡) ==> (≡)) IMsg.
+  Proof. by intros ???. Qed.
+End imsg_ofe.
+
+Program Definition iMsg_base_def {Σ V}
+    (v : V) (P : iProp Σ) (p : iProto Σ V) : iMsg Σ V :=
+  IMsg (λ v', λne p', ⌜ v = v' ⌝ ∗ Next p ≡ p' ∗ P)%I.
+Next Obligation. solve_proper. Qed.
+Definition iMsg_base_aux : seal (@iMsg_base_def). by eexists. Qed.
+Definition iMsg_base := iMsg_base_aux.(unseal).
+Definition iMsg_base_eq : @iMsg_base = @iMsg_base_def := iMsg_base_aux.(seal_eq).
+Arguments iMsg_base {_ _} _%V _%I _%proto.
+Instance: Params (@iMsg_base) 3 := {}.
+
+Program Definition iMsg_exist_def {Σ V A} (m : A → iMsg Σ V) : iMsg Σ V :=
+  IMsg (λ v', λne p', ∃ x, m x v' p')%I.
+Next Obligation. solve_proper. Qed.
+Definition iMsg_exist_aux : seal (@iMsg_exist_def). by eexists. Qed.
+Definition iMsg_exist := iMsg_exist_aux.(unseal).
+Definition iMsg_exist_eq : @iMsg_exist = @iMsg_exist_def := iMsg_exist_aux.(seal_eq).
+Arguments iMsg_exist {_ _ _} _%msg.
+Instance: Params (@iMsg_exist) 3 := {}.
+
+Definition iMsg_texist {Σ V} {TT : tele} (m : TT → iMsg Σ V) : iMsg Σ V :=
+  tele_fold (@iMsg_exist Σ V) (λ x, x) (tele_bind m).
+Arguments iMsg_texist {_ _ !_} _%msg /.
+
+Notation "'MSG' v {{ P } } ; p" := (iMsg_base v P p)
+  (at level 200, v at level 20, right associativity,
+   format "MSG  v  {{  P  } } ;  p") : msg_scope.
+Notation "'MSG' v ; p" := (iMsg_base v True p)
+  (at level 200, v at level 20, right associativity,
+   format "MSG  v ;  p") : msg_scope.
+Notation "∃ x .. y , m" :=
+  (iMsg_exist (λ x, .. (iMsg_exist (λ y, m)) ..)%msg) : msg_scope.
+Notation "'∃..' x .. y , m" :=
+  (iMsg_texist (λ x, .. (iMsg_texist (λ y, m)) .. )%msg)
+  (at level 200, x binder, y binder, right associativity,
+   format "∃..  x  ..  y ,  m") : msg_scope.
 
 (** * Operators *)
 Definition iProto_end_def {Σ V} : iProto Σ V := proto_end.
@@ -56,119 +130,64 @@ Definition iProto_end := iProto_end_aux.(unseal).
 Definition iProto_end_eq : @iProto_end = @iProto_end_def := iProto_end_aux.(seal_eq).
 Arguments iProto_end {_ _}.
 
-Program Definition iProto_message_def {Σ V} {TT : tele} (a : action)
-    (pc : TT → V * iProp Σ * iProto Σ V) : iProto Σ V :=
-  proto_message a (λ v, λne p', ∃ x : TT,
-    ⌜ v = (pc x).1.1 ⌝ ∗
-    (pc x).1.2 ∗
-    p' ≡ (pc x).2)%I.
-Next Obligation. solve_proper. Qed.
+Definition iProto_message_def {Σ V} (a : action) (m : iMsg Σ V) : iProto Σ V :=
+  proto_message a m.
 Definition iProto_message_aux : seal (@iProto_message_def). by eexists. Qed.
 Definition iProto_message := iProto_message_aux.(unseal).
 Definition iProto_message_eq :
   @iProto_message = @iProto_message_def := iProto_message_aux.(seal_eq).
-Arguments iProto_message {_ _ _} _ _%proto.
-Instance: Params (@iProto_message) 4 := {}.
-
-Notation "< a > x1 .. xn , 'MSG' v {{ P } } ; p" :=
-  (iProto_message
-    a
-    (tele_app (TT:=TeleS (λ x1, .. (TeleS (λ xn, TeleO)) .. )) $
-                       λ x1, .. (λ xn, (v%V,P%I,p%proto)) ..))
-  (at level 20, a at level 10, x1 binder, xn binder,
-   v at level 20, P, p at level 200) : proto_scope.
-Notation "< a > x1 .. xn , 'MSG' v ; p" :=
-  (iProto_message
-    a
-    (tele_app (TT:=TeleS (λ x1, .. (TeleS (λ xn, TeleO)) .. )) $
-                       λ x1, .. (λ xn, (v%V,True%I,p%proto)) ..))
-  (at level 20, a at level 10, x1 binder, xn binder,
-   v at level 20, p at level 200) : proto_scope.
-Notation "< a > 'MSG' v {{ P } } ; p" :=
-  (iProto_message
-    a
-    (tele_app (TT:=TeleO) (v%V,P%I,p%proto)))
-  (at level 20, a at level 10, v at level 20, P, p at level 200) : proto_scope.
-Notation "< a > 'MSG' v ; p" :=
-  (iProto_message
-    a
-    (tele_app (TT:=TeleO) (v%V,True%I,p%proto)))
-  (at level 20, a at level 10, v at level 20, p at level 200) : proto_scope.
-
-Notation "<!> x1 .. xn , 'MSG' v {{ P } } ; p" :=
-  (iProto_message
-    Send
-    (tele_app (TT:=TeleS (λ x1, .. (TeleS (λ xn, TeleO)) .. )) $
-                       λ x1, .. (λ xn, (v%V,P%I,p%proto)) ..))
-  (at level 20, x1 binder, xn binder, v at level 20, P, p at level 200) : proto_scope.
-Notation "<!> x1 .. xn , 'MSG' v ; p" :=
-  (iProto_message
-    Send
-    (tele_app (TT:=TeleS (λ x1, .. (TeleS (λ xn, TeleO)) .. )) $
-                       λ x1, .. (λ xn, (v%V,True%I,p%proto)) ..))
-  (at level 20, x1 binder, xn binder, v at level 20, p at level 200) : proto_scope.
-Notation "<!> 'MSG' v {{ P } } ; p" :=
-  (iProto_message
-    (TT:=TeleO)
-    Send
-    (tele_app (TT:=TeleO) (v%V,P%I,p%proto)))
-  (at level 20, v at level 20, P, p at level 200) : proto_scope.
-Notation "<!> 'MSG' v ; p" :=
-  (iProto_message
-    (TT:=TeleO)
-    Send
-    (tele_app (TT:=TeleO) (v%V,True%I,p%proto)))
-  (at level 20, v at level 20, p at level 200) : proto_scope.
-
-Notation "<?> x1 .. xn , 'MSG' v {{ P } } ; p" :=
-  (iProto_message
-    Recv
-    (tele_app (TT:=TeleS (λ x1, .. (TeleS (λ xn, TeleO)) .. )) $
-                       λ x1, .. (λ xn, (v%V,P%I,p%proto)) ..))
-  (at level 20, x1 binder, xn binder, v at level 20, P, p at level 200) : proto_scope.
-Notation "<?> x1 .. xn , 'MSG' v ; p" :=
-  (iProto_message
-    Recv
-    (tele_app (TT:=TeleS (λ x1, .. (TeleS (λ xn, TeleO)) .. )) $
-                       λ x1, .. (λ xn, (v%V,True%I,p%proto)) ..))
-  (at level 20, x1 binder, xn binder, v at level 20, p at level 200) : proto_scope.
-Notation "<?> 'MSG' v {{ P } } ; p" :=
-  (iProto_message
-    Recv
-    (tele_app (TT:=TeleO) (v%V,P%I,p%proto)))
-  (at level 20, v at level 20, P, p at level 200) : proto_scope.
-Notation "<?> 'MSG' v ; p" :=
-  (iProto_message
-    Recv
-    (tele_app (TT:=TeleO) (v%V,True%I,p%proto)))
-  (at level 20, v at level 20, p at level 200) : proto_scope.
+Arguments iProto_message {_ _} _ _%msg.
+Instance: Params (@iProto_message) 3 := {}.
 
 Notation "'END'" := iProto_end : proto_scope.
 
+Notation "< a > m" := (iProto_message a m)
+  (at level 200, a at level 10, m at level 200,
+   format "< a >  m") : proto_scope.
+Notation "< a @ x1 .. xn > m" := (iProto_message a (∃ x1, .. (∃ xn, m) ..))
+  (at level 200, a at level 10, x1 closed binder, xn closed binder, m at level 200,
+   format "< a  @  x1  ..  xn >  m") : proto_scope.
+Notation "< a @.. x1 .. xn > m" := (iProto_message a (∃.. x1, .. (∃.. xn, m) ..))
+  (at level 200, a at level 10, x1 closed binder, xn closed binder, m at level 200,
+   format "< a  @..  x1  ..  xn >  m") : proto_scope.
+
+Notation "<!> m" := (<Send> m) (at level 200, m at level 200) : proto_scope.
+Notation "<! x1 .. xn > m" := (<!> ∃ x1, .. (∃ xn, m) ..)
+  (at level 200, x1 closed binder, xn closed binder, m at level 200,
+   format "<!  x1  ..  xn >  m") : proto_scope.
+Notation "<!.. x1 .. xn > m" := (<!> ∃.. x1, .. (∃.. xn, m) ..)
+  (at level 200, x1 closed binder, xn closed binder, m at level 200,
+   format "<!..  x1  ..  xn >  m") : proto_scope.
+
+Notation "<?> m" := (<Recv> m) (at level 200, m at level 200) : proto_scope.
+Notation "<? x1 .. xn > m" := (<?> ∃ x1, .. (∃ xn, m) ..)
+  (at level 200, x1 closed binder, xn closed binder, m at level 200,
+   format "<?  x1  ..  xn >  m") : proto_scope.
+Notation "<?.. x1 .. xn > m" := (<?> ∃.. x1, .. (∃.. xn, m) ..)
+  (at level 200, x1 closed binder, xn closed binder, m at level 200,
+   format "<?..  x1  ..  xn >  m") : proto_scope.
+
 (** * Operations *)
-Program Definition iProto_map_app_cont {Σ V}
-    (rec : iProto Σ V → iProto Σ V) (pc : iProto Σ V -n> iPropO Σ) :
-    iProto Σ V -n> iPropO Σ :=
-  λne p1', (∃ p1, pc p1 ∗ p1' ≡ rec p1)%I.
+Program Definition iMsg_map {Σ V}
+    (rec : iProto Σ V → iProto Σ V) (m : iMsg Σ V) : iMsg Σ V :=
+  IMsg (λ v, λne p1', ∃ p1, m v (Next p1) ∗ p1' ≡ Next (rec p1))%I.
 Next Obligation. solve_proper. Qed.
 
 Program Definition iProto_map_app_aux {Σ V}
     (f : action → action) (p2 : iProto Σ V)
     (rec : iProto Σ V -n> iProto Σ V) : iProto Σ V -n> iProto Σ V := λne p,
-  proto_elim p2 (λ a pc,
-    proto_message (f a) (iProto_map_app_cont rec ∘ pc)) p.
+  proto_elim p2 (λ a m,
+    proto_message (f a) (iMsg_map rec (IMsg m))) p.
 Next Obligation.
-  intros Σ V f p2 rec n p1 p1' Hp. apply proto_elim_ne=> // a pc1 pc2 Hpc.
-  apply proto_message_contractive; destruct n as [|n]=> // v p'; simpl in *.
-  by repeat f_equiv.
+  intros Σ V f p2 rec n p1 p1' Hp. apply proto_elim_ne=> // a m1 m2 Hm.
+  apply proto_message_ne=> v p' /=. by repeat f_equiv.
 Qed.
 
 Instance iProto_map_app_aux_contractive {Σ V} f (p2 : iProto Σ V) :
   Contractive (iProto_map_app_aux f p2).
 Proof.
-  intros n rec1 rec2 Hrec p1; simpl. apply proto_elim_ne=> // a pc1 pc2 Hpc.
-  apply proto_message_contractive; destruct n as [|n]=> // v p'; simpl in *.
-  by repeat f_equiv.
+  intros n rec1 rec2 Hrec p1; simpl. apply proto_elim_ne=> // a m1 m2 Hm.
+  apply proto_message_ne=> v p' /=. by repeat (f_contractive || f_equiv).
 Qed.
 
 Definition iProto_map_app {Σ V} (f : action → action)
@@ -183,6 +202,7 @@ Definition iProto_app_eq : @iProto_app = @iProto_app_def := iProto_app_aux.(seal
 Arguments iProto_app {_ _} _%proto _%proto.
 Instance: Params (@iProto_app) 2 := {}.
 Infix "<++>" := iProto_app (at level 60) : proto_scope.
+Notation "m <++> p" := (iMsg_map (flip iProto_app p) m) : msg_scope.
 
 Definition iProto_dual_def {Σ V} (p : iProto Σ V) : iProto Σ V :=
   iProto_map_app action_dual proto_end p.
@@ -192,6 +212,8 @@ Definition iProto_dual_eq :
   @iProto_dual = @iProto_dual_def := iProto_dual_aux.(seal_eq).
 Arguments iProto_dual {_ _} _%proto.
 Instance: Params (@iProto_dual) 2 := {}.
+Notation iMsg_dual := (iMsg_map iProto_dual).
+
 Definition iProto_dual_if {Σ V} (d : bool) (p : iProto Σ V) : iProto Σ V :=
   if d then iProto_dual p else p.
 Arguments iProto_dual_if {_ _} _ _%proto.
@@ -219,19 +241,16 @@ Example:
 *)
 Definition iProto_le_pre {Σ V}
     (rec : iProto Σ V → iProto Σ V → iProp Σ) (p1 p2 : iProto Σ V) : iProp Σ :=
-  (p1 ≡ proto_end ∗ p2 ≡ proto_end) ∨
-  ∃ a1 a2 pc1 pc2,
-    p1 ≡ proto_message a1 pc1 ∗
-    p2 ≡ proto_message a2 pc2 ∗
+  ◇ (p1 ≡ END ∗ p2 ≡ END) ∨
+  ∃ a1 a2 m1 m2,
+    ◇ (p1 ≡ <a1> m1) ∗ ◇ (p2 ≡ <a2> m2) ∗
     match a1, a2 with
-    | Recv, Recv => ▷ ∀ v p1', pc1 v p1' -∗ ∃ p2', rec p1' p2' ∗ pc2 v p2'
-    | Send, Send => ▷ ∀ v p2', pc2 v p2' -∗ ∃ p1', rec p1' p2' ∗ pc1 v p1'
-    | Recv, Send => ▷ ∀ v1 v2 p1' p2',
-       pc1 v1 p1' -∗ pc2 v2 p2' -∗ ∃ pc1' pc2' pt,
-         rec p1' (proto_message Send pc1') ∗
-         rec (proto_message Recv pc2') p2' ∗
-         pc1' v2 pt ∗
-         pc2' v1 pt
+    | Recv, Recv => ∀ v p1', m1 v (Next p1') -∗ ◇ ∃ p2', ▷ rec p1' p2' ∗ m2 v (Next p2')
+    | Send, Send => ∀ v p2', m2 v (Next p2') -∗ ◇ ∃ p1', ▷ rec p1' p2' ∗ m1 v (Next p1')
+    | Recv, Send => ∀ v1 v2 p1' p2',
+       m1 v1 (Next p1') -∗ m2 v2 (Next p2') -∗ ◇ ∃ m1' m2' pt,
+         ▷ rec p1' (<!> m1') ∗ ▷ rec (<?> m2') p2' ∗
+         m1' v2 (Next pt) ∗ m2' v1 (Next pt)
     | Send, Recv => False
     end.
 Instance iProto_le_pre_ne {Σ V} (rec : iProto Σ V → iProto Σ V → iProp Σ) :
@@ -252,6 +271,7 @@ Definition iProto_le {Σ V} (p1 p2 : iProto Σ V) : iProp Σ :=
   fixpoint iProto_le_pre' p1 p2.
 Arguments iProto_le {_ _} _%proto _%proto.
 Instance: Params (@iProto_le) 2 := {}.
+Notation "p ⊑ q" := (iProto_le p q) : bi_scope.
 
 Fixpoint iProto_interp_aux {Σ V} (n : nat)
     (vsl vsr : list V) (pl pr : iProto Σ V) : iProp Σ :=
@@ -259,18 +279,18 @@ Fixpoint iProto_interp_aux {Σ V} (n : nat)
   | 0 => ∃ p,
      ⌜ vsl = [] ⌝ ∗
      ⌜ vsr = [] ⌝ ∗
-     iProto_le p pl ∗
-     iProto_le (iProto_dual p) pr
+     p ⊑ pl ∗
+     iProto_dual p ⊑ pr
   | S n =>
-     (∃ vl vsl' pc p2',
+     (∃ vl vsl' m p2',
        ⌜ vsl = vl :: vsl' ⌝ ∗
-       iProto_le (proto_message Recv pc) pr ∗
-       pc vl p2' ∗
+       (<?> m) ⊑ pr ∗
+       m vl (Next p2') ∗
        iProto_interp_aux n vsl' vsr pl p2') ∨
-     (∃ vr vsr' pc p1',
+     (∃ vr vsr' m p1',
        ⌜ vsr = vr :: vsr' ⌝ ∗
-       iProto_le (proto_message Recv pc) pl ∗
-       pc vr p1' ∗
+       (<?> m) ⊑ pl ∗
+       m vr (Next p1') ∗
        iProto_interp_aux n vsl vsr' p1' pr)
   end.
 Definition iProto_interp {Σ V} (vsl vsr : list V) (pl pr : iProto Σ V) : iProp Σ :=
@@ -319,46 +339,72 @@ Definition iProto_ctx `{protoG Σ V}
 (** * The connective for ownership of channel ends *)
 Definition iProto_own `{!protoG Σ V}
     (γ : proto_name) (s : side) (p : iProto Σ V) : iProp Σ :=
-  ∃ p', ▷ iProto_le p' p ∗ iProto_own_frag γ s p'.
+  ∃ p', ▷ (p' ⊑ p) ∗ iProto_own_frag γ s p'.
 Arguments iProto_own {_ _ _} _ _%proto.
 Instance: Params (@iProto_own) 3 := {}.
 
 (** * Proofs *)
 Section proto.
   Context `{!protoG Σ V}.
+  Implicit Types v : V.
   Implicit Types p pl pr : iProto Σ V.
-  Implicit Types TT : tele.
+  Implicit Types m : iMsg Σ V.
+
+  (** ** Equality *)
+  Lemma iProto_case p : p ≡ END ∨ ∃ a m, p ≡ <a> m.
+  Proof.
+    rewrite iProto_message_eq iProto_end_eq.
+    destruct (proto_case p) as [|(a&m&?)]; [by left|right].
+    by exists a, (IMsg m).
+  Qed.
+  Lemma iProto_message_equivI {SPROP : sbi} a1 a2 m1 m2 :
+    (<a1> m1) ≡ (<a2> m2) ⊣⊢@{SPROP} ⌜ a1 = a2 ⌝ ∧ (∀ v lp, m1 v lp ≡ m2 v lp).
+  Proof. rewrite iProto_message_eq. apply proto_message_equivI. Qed.
+  Lemma iProto_message_end_equivI {SPROP : sbi} a m : (<a> m) ≡ END ⊢@{SPROP} False.
+  Proof. rewrite iProto_message_eq iProto_end_eq. apply proto_message_end_equivI. Qed.
+  Lemma iProto_end_message_equivI {SPROP : sbi} a m : END ≡ (<a> m) ⊢@{SPROP} False.
+  Proof. by rewrite bi.internal_eq_sym iProto_message_end_equivI. Qed.
 
   (** ** Non-expansiveness of operators *)
-  Lemma iProto_message_contractive {TT} a
-      (pc1 pc2 : TT → V * iProp Σ * iProto Σ V) n :
-    (∀.. x, (pc1 x).1.1 = (pc2 x).1.1) →
-    (∀.. x, dist_later n ((pc1 x).1.2) ((pc2 x).1.2)) →
-    (∀.. x, dist_later n ((pc1 x).2) ((pc2 x).2)) →
-    iProto_message a pc1 ≡{n}≡ iProto_message a pc2.
+  Global Instance iMsg_contractive v n :
+    Proper (dist n ==> dist_later n ==> dist n) (iMsg_base (Σ:=Σ) (V:=V) v).
+  Proof. rewrite iMsg_base_eq. solve_proper. Qed.
+  Global Instance iMsg_ne v : NonExpansive2 (iMsg_base (Σ:=Σ) (V:=V) v).
+  Proof. rewrite iMsg_base_eq. solve_proper. Qed.
+  Global Instance iMsg_proper v :
+    Proper ((≡) ==> (≡) ==> (≡)) (iMsg_base (Σ:=Σ) (V:=V) v).
+  Proof. apply (ne_proper_2 _). Qed.
+
+  Global Instance iMsg_exist_ne A n :
+    Proper (pointwise_relation _ (dist n) ==> (dist n)) (@iMsg_exist Σ V A).
+  Proof. rewrite iMsg_exist_eq. solve_proper. Qed.
+  Global Instance iMsg_exist_proper A :
+    Proper (pointwise_relation _ (≡) ==> (≡)) (@iMsg_exist Σ V A).
+  Proof. rewrite iMsg_exist_eq. solve_proper. Qed.
+
+  Global Instance iProto_message_ne a :
+    NonExpansive (iProto_message (Σ:=Σ) (V:=V) a).
+  Proof. rewrite iProto_message_eq. solve_proper. Qed.
+  Global Instance iProto_message_proper a :
+    Proper ((≡) ==> (≡)) (iProto_message (Σ:=Σ) (V:=V) a).
+  Proof. apply (ne_proper _). Qed.
+
+  (** Helpers *)
+  Lemma iMsg_map_base f v P p :
+    NonExpansive f →
+    iMsg_map f (MSG v {{ P }}; p) ≡ (MSG v {{ P }}; f p)%msg.
   Proof.
-    rewrite !tforall_forall=> Hv HP Hp.
-    rewrite iProto_message_eq /iProto_message_def.
-    apply proto_message_contractive; destruct n as [|n]=> // v f /=.
-    repeat (apply Hv || apply HP || apply Hp || f_contractive || f_equiv).
+    rewrite iMsg_base_eq. intros ? v' p'; simpl. iSplit.
+    - iDestruct 1 as (p'') "[(->&Hp&$) Hp']". iSplit; [done|].
+      iRewrite "Hp'". iIntros "!>". by iRewrite "Hp".
+    - iIntros "(->&Hp'&$)". iExists p. iRewrite -"Hp'". auto.
   Qed.
-  Lemma iProto_message_ne {TT} a (pc1 pc2 : TT → V * iProp Σ * iProto Σ V) n :
-    (∀.. x, (pc1 x).1.1 = (pc2 x).1.1) →
-    (∀.. x, (pc1 x).1.2 ≡{n}≡ (pc2 x).1.2) →
-    (∀.. x, (pc1 x).2 ≡{n}≡ (pc2 x).2) →
-    iProto_message a pc1 ≡{n}≡ iProto_message a pc2.
+  Lemma iMsg_map_exist {A} f (m : A → iMsg Σ V) :
+    iMsg_map f (∃ x, m x) ≡ (∃ x, iMsg_map f (m x))%msg.
   Proof.
-    rewrite !tforall_forall=> Hv HP Hp.
-    apply iProto_message_contractive; apply tforall_forall; eauto using dist_dist_later.
-  Qed.
-  Lemma iProto_message_proper {TT} a (pc1 pc2 : TT → V * iProp Σ * iProto Σ V) :
-    (∀.. x, (pc1 x).1.1 = (pc2 x).1.1) →
-    (∀.. x, (pc1 x).1.2 ≡ (pc2 x).1.2) →
-    (∀.. x, (pc1 x).2 ≡ (pc2 x).2) →
-    iProto_message a pc1 ≡ iProto_message a pc2.
-  Proof.
-    rewrite !tforall_forall=> Hv HP Hp. apply equiv_dist => n.
-    apply iProto_message_ne; apply tforall_forall=> x; by try apply equiv_dist.
+    rewrite iMsg_exist_eq. intros v' p'; simpl. iSplit.
+    - iDestruct 1 as (p'') "[H Hp']". iDestruct "H" as (x) "H"; auto.
+    - iDestruct 1 as (x p'') "[Hm Hp']". auto.
   Qed.
 
   (** ** Dual *)
@@ -372,71 +418,54 @@ Section proto.
     Proper ((≡) ==> (≡)) (@iProto_dual_if Σ V d).
   Proof. apply (ne_proper _). Qed.
 
-  Lemma iProto_dual_end' : iProto_dual (Σ:=Σ) (V:=V) proto_end ≡ proto_end.
+  Lemma iProto_dual_end : iProto_dual (Σ:=Σ) (V:=V) END ≡ END.
   Proof.
-    rewrite iProto_dual_eq /iProto_dual_def /iProto_map_app.
+    rewrite iProto_end_eq iProto_dual_eq /iProto_dual_def /iProto_map_app.
     etrans; [apply (fixpoint_unfold (iProto_map_app_aux _ _))|]; simpl.
     by rewrite proto_elim_end.
   Qed.
-  Lemma iProto_dual_message' a pc :
-    iProto_dual (Σ:=Σ) (V:=V) (proto_message a pc)
-    ≡ proto_message (action_dual a) (iProto_map_app_cont iProto_dual ∘ pc).
+  Lemma iProto_dual_message a m :
+    iProto_dual (<a> m) ≡ <action_dual a> iMsg_dual m.
   Proof.
-    rewrite iProto_dual_eq /iProto_dual_def /iProto_map_app.
+    rewrite iProto_message_eq iProto_dual_eq /iProto_dual_def /iProto_map_app.
     etrans; [apply (fixpoint_unfold (iProto_map_app_aux _ _))|]; simpl.
-    apply: proto_elim_message=> a' pc1 pc2 Hpc; f_equiv; solve_proper.
+    apply: proto_elim_message=> a' m1 m2 Hm; f_equiv; solve_proper.
   Qed.
-
-  Lemma iProto_dual_end : iProto_dual (Σ:=Σ) (V:=V) END ≡ END%proto.
-  Proof. rewrite iProto_end_eq. apply iProto_dual_end'. Qed.
-
-  Lemma iProto_dual_message {TT} a (pc : TT → V * iProp Σ * iProto Σ V) :
-    iProto_dual (iProto_message a pc)
-    ≡ iProto_message (action_dual a) (prod_map id iProto_dual ∘ pc).
-  Proof.
-    rewrite iProto_message_eq /iProto_message_def iProto_dual_message' /=.
-    do 2 f_equiv; intros p'; simpl. iSplit.
-    - iDestruct 1 as (pd) "[H Hp']". iDestruct "H" as (x ->) "[Hpc Hpd]".
-      iExists x. iSplit; [done|]; iFrame. iRewrite "Hp'". by iRewrite "Hpd".
-    - iDestruct 1 as (x ->) "[Hpc Hpd]"; auto 10.
-  Qed.
-
-  Lemma iProto_dual_message_tele {TT} a (pc : TT -t> V * iProp Σ * iProto Σ V) :
-    iProto_dual (iProto_message a (tele_app pc))
-    ≡ iProto_message (action_dual a) (tele_app (tele_map (prod_map id iProto_dual) pc)).
-  Proof.
-    rewrite iProto_dual_message.
-    apply iProto_message_proper; apply tforall_forall=> x; by rewrite /=?tele_map_app.
-  Qed.
+  Lemma iMsg_dual_base v P p :
+    iMsg_dual (MSG v {{ P }}; p) ≡ (MSG v {{ P }}; iProto_dual p)%msg.
+  Proof. apply iMsg_map_base, _. Qed.
+  Lemma iMsg_dual_exist {A} (m : A → iMsg Σ V) :
+    iMsg_dual (∃ x, m x) ≡ (∃ x, iMsg_dual (m x))%msg.
+  Proof. apply iMsg_map_exist. Qed.
 
   Global Instance iProto_dual_involutive : Involutive (≡) (@iProto_dual Σ V).
   Proof.
     intros p. apply (uPred.internal_eq_soundness (M:=iResUR Σ)).
-    iLöb as "IH" forall (p). destruct (proto_case p) as [->|(a&pc&->)].
-    { by rewrite !iProto_dual_end'. }
-    rewrite !iProto_dual_message' involutive.
-    iApply proto_message_equivI; iSplit; [done|]; iIntros (v p') "/=".
-    iIntros "!>"; iApply prop_ext; iIntros "!>"; iSplit.
+    iLöb as "IH" forall (p). destruct (iProto_case p) as [->|(a&m&->)].
+    { by rewrite !iProto_dual_end. }
+    rewrite !iProto_dual_message involutive.
+    iApply iProto_message_equivI; iSplit; [done|]; iIntros (v p') "/=".
+    iApply prop_ext; iIntros "!>"; iSplit.
     - iDestruct 1 as (pd) "[H Hp']". iRewrite "Hp'".
-      iDestruct "H" as (pdd) "[H Hpd]". iRewrite "Hpd". by iRewrite ("IH" $! pdd).
-    - iIntros "H". iExists (iProto_dual p').
-      iSplitL; [by auto|]. by iRewrite ("IH" $! p').
+      iDestruct "H" as (pdd) "[H #Hpd]".
+      iApply (bi.internal_eq_rewrite); [|done]; iIntros "!>".
+      iRewrite "Hpd". by iRewrite ("IH" $! pdd).
+    - iIntros "H". destruct (Next_uninj p') as [p'' Hp']. iExists _.
+      rewrite Hp'. iSplitL; [by auto|]. iIntros "!>". by iRewrite ("IH" $! p'').
   Qed.
 
   (** ** Append *)
-  Lemma iProto_app_end' p : (proto_end <++> p)%proto ≡ p.
+  Global Instance iProto_app_end_l : LeftId (≡) END (@iProto_app Σ V).
   Proof.
-    rewrite iProto_app_eq /iProto_app_def /iProto_map_app.
+    intros p. rewrite iProto_end_eq iProto_app_eq /iProto_app_def /iProto_map_app.
     etrans; [apply (fixpoint_unfold (iProto_map_app_aux _ _))|]; simpl.
     by rewrite proto_elim_end.
   Qed.
-  Lemma iProto_app_message' a pc p2 :
-    (proto_message a pc <++> p2)%proto
-    ≡ proto_message a (iProto_map_app_cont (flip iProto_app p2) ∘ pc).
+  Lemma iProto_app_message a m p2 : (<a> m) <++> p2 ≡ <a> m <++> p2.
   Proof.
-    rewrite iProto_app_eq /iProto_app_def /iProto_map_app.
+    rewrite iProto_message_eq iProto_app_eq /iProto_app_def /iProto_map_app.
     etrans; [apply (fixpoint_unfold (iProto_map_app_aux _ _))|]; simpl.
-    apply: proto_elim_message => a' pc1 pc2 Hpc. f_equiv; solve_proper.
+    apply: proto_elim_message=> a' m1 m2 Hm. f_equiv; solve_proper.
   Qed.
 
   Global Instance iProto_app_ne : NonExpansive2 (@iProto_app Σ V).
@@ -447,326 +476,411 @@ Section proto.
     { intros p1 p1' Hp1 p2 p2' <-. by rewrite iProto_app_eq /iProto_app_def Hp1. }
     intros n p1 p1' Hp1 p2 p2' Hp2. rewrite Hp1. clear p1 Hp1.
     revert p1'. induction (lt_wf n) as [n _ IH]; intros p1.
-    destruct (proto_case p1) as [->|(a&pc&->)].
-    { by rewrite !iProto_app_end'. }
-    rewrite !iProto_app_message'.
-    apply proto_message_contractive; destruct n as [|n]=> // v p' /=.
-    do 4 f_equiv. apply IH; eauto using dist_le with lia.
+    destruct (iProto_case p1) as [->|(a&m&->)].
+    { by rewrite !left_id. }
+    rewrite !iProto_app_message. f_equiv=> v p' /=. do 4 f_equiv.
+    f_contractive. apply IH; eauto using dist_le with lia.
   Qed.
   Global Instance iProto_app_proper : Proper ((≡) ==> (≡) ==> (≡)) (@iProto_app Σ V).
   Proof. apply (ne_proper_2 _). Qed.
 
-  Lemma iProto_app_message {TT} a (pc : TT → V * iProp Σ * iProto Σ V) p2 :
-    (iProto_message a pc <++> p2)%proto
-    ≡ iProto_message a (prod_map id (flip iProto_app p2) ∘ pc).
-  Proof.
-    rewrite iProto_message_eq /iProto_message_def iProto_app_message' /=.
-    f_equiv=> v ps /=. iSplit.
-    - iDestruct 1 as (p1') "[H Hps]". iDestruct "H" as (x ->) "[Hpc #Hp1']".
-      iExists x. iSplit; [done|]. iFrame. iRewrite "Hps". by iRewrite "Hp1'".
-    - iDestruct 1 as (x ->) "[Hpc Hps]". auto 10.
-  Qed.
+  Lemma iMsg_app_base v P p1 p2 :
+    ((MSG v {{ P }}; p1) <++> p2)%msg ≡ (MSG v {{ P }}; p1 <++> p2)%msg.
+  Proof. apply: iMsg_map_base. Qed.
+  Lemma iMsg_app_exist {A} (m : A → iMsg Σ V) p2 :
+    ((∃ x, m x) <++> p2)%msg ≡ (∃ x, m x <++> p2)%msg.
+  Proof. apply iMsg_map_exist. Qed.
 
-  Lemma iProto_app_message_tele {TT} a (pc : TT -t> V * iProp Σ * iProto Σ V) p2 :
-    (iProto_message a (tele_app pc) <++> p2)%proto
-    ≡ iProto_message a (tele_app (tele_map (prod_map id (flip iProto_app p2)) pc)).
+  Global Instance iProto_app_end_r : RightId (≡) END (@iProto_app Σ V).
   Proof.
-    rewrite iProto_app_message.
-    apply iProto_message_proper; apply tforall_forall=> x; by rewrite /=?tele_map_app.
-  Qed.
-
-  Global Instance iProto_app_end_l : LeftId (≡) END%proto (@iProto_app Σ V).
-  Proof. intros p. by rewrite iProto_end_eq /iProto_end_def iProto_app_end'. Qed.
-  Global Instance iProto_app_end_r : RightId (≡) END%proto (@iProto_app Σ V).
-  Proof.
-    rewrite iProto_end_eq /iProto_end_def.
     intros p. apply (uPred.internal_eq_soundness (M:=iResUR Σ)).
-    iLöb as "IH" forall (p). destruct (proto_case p) as [->|(a&pc&->)].
-    { by rewrite iProto_app_end'. }
-    rewrite iProto_app_message'.
-    iApply proto_message_equivI; iSplit; [done|]; iIntros (v p') "/=".
-    iIntros "!>". iApply prop_ext; iIntros "!>". iSplit.
-    - iDestruct 1 as (p1') "[H Hp']". iRewrite "Hp'". by iRewrite ("IH" $! p1').
-    - iIntros "H". iExists p'. iFrame "H". by iRewrite ("IH" $! p').
+    iLöb as "IH" forall (p). destruct (iProto_case p) as [->|(a&m&->)].
+    { by rewrite left_id. }
+    rewrite iProto_app_message.
+    iApply iProto_message_equivI; iSplit; [done|]; iIntros (v p') "/=".
+    iApply prop_ext; iIntros "!>". iSplit.
+    - iDestruct 1 as (p1') "[H Hp']". iRewrite "Hp'".
+      iApply (bi.internal_eq_rewrite); [|done]; iIntros "!>".
+      by iRewrite ("IH" $! p1').
+    - iIntros "H". destruct (Next_uninj p') as [p'' Hp']. iExists p''.
+      rewrite Hp'. iSplitL; [by auto|]. iIntros "!>". by iRewrite ("IH" $! p'').
   Qed.
   Global Instance iProto_app_assoc : Assoc (≡) (@iProto_app Σ V).
   Proof.
     intros p1 p2 p3. apply (uPred.internal_eq_soundness (M:=iResUR Σ)).
-    iLöb as "IH" forall (p1). destruct (proto_case p1) as [->|(a&pc&->)].
-    { by rewrite !iProto_app_end'. }
-    rewrite !iProto_app_message'.
-    iApply proto_message_equivI; iSplit; [done|]; iIntros (v p123) "/=".
-    iIntros "!>". iApply prop_ext; iIntros "!>". iSplit.
+    iLöb as "IH" forall (p1). destruct (iProto_case p1) as [->|(a&m&->)].
+    { by rewrite !left_id. }
+    rewrite !iProto_app_message.
+    iApply iProto_message_equivI; iSplit; [done|]; iIntros (v p123) "/=".
+    iApply prop_ext; iIntros "!>". iSplit.
     - iDestruct 1 as (p1') "[H #Hp']".
-      iExists (p1' <++> p2)%proto. iSplitL; [by auto|].
-      iRewrite "Hp'". iApply "IH".
+      iExists (p1' <++> p2). iSplitL; [by auto|].
+      iRewrite "Hp'". iIntros "!>". iApply "IH".
     - iDestruct 1 as (p12) "[H #Hp123]". iDestruct "H" as (p1') "[H #Hp12]".
       iExists p1'. iFrame "H". iRewrite "Hp123".
-      iRewrite "Hp12". by iRewrite ("IH" $! p1').
+      iIntros "!>". iRewrite "Hp12". by iRewrite ("IH" $! p1').
   Qed.
 
   Lemma iProto_dual_app p1 p2 :
-    iProto_dual (p1 <++> p2) ≡ (iProto_dual p1 <++> iProto_dual p2)%proto.
+    iProto_dual (p1 <++> p2) ≡ iProto_dual p1 <++> iProto_dual p2.
   Proof.
     apply (uPred.internal_eq_soundness (M:=iResUR Σ)).
-    iLöb as "IH" forall (p1 p2). destruct (proto_case p1) as [->|(a&pc&->)].
-    { by rewrite iProto_dual_end' !iProto_app_end'. }
-    rewrite iProto_dual_message' !iProto_app_message' iProto_dual_message' /=.
-    iApply proto_message_equivI; iSplit; [done|]; iIntros (v p12) "/=".
-    iIntros "!>"; iApply prop_ext; iIntros "!>". iSplit.
+    iLöb as "IH" forall (p1 p2). destruct (iProto_case p1) as [->|(a&m&->)].
+    { by rewrite iProto_dual_end !left_id. }
+    rewrite iProto_dual_message !iProto_app_message iProto_dual_message /=.
+    iApply iProto_message_equivI; iSplit; [done|]; iIntros (v p12) "/=".
+    iApply prop_ext; iIntros "!>". iSplit.
     - iDestruct 1 as (p12d) "[H #Hp12]". iDestruct "H" as (p1') "[H #Hp12d]".
       iExists (iProto_dual p1'). iSplitL; [by auto|].
-      iRewrite "Hp12". iRewrite "Hp12d". iApply "IH".
+      iRewrite "Hp12". iIntros "!>". iRewrite "Hp12d". iApply "IH".
     - iDestruct 1 as (p1') "[H #Hp12]". iDestruct "H" as (p1d) "[H #Hp1']".
-      iExists (p1d <++> p2)%proto. iSplitL; [by auto|].
-      iRewrite "Hp12". iRewrite "Hp1'". by iRewrite ("IH" $! p1d p2).
+      iExists (p1d <++> p2). iSplitL; [by auto|].
+      iRewrite "Hp12". iIntros "!>". iRewrite "Hp1'". by iRewrite ("IH" $! p1d p2).
   Qed.
 
   (** ** Protocol entailment **)
+  Lemma iProto_le_unfold p1 p2 : iProto_le p1 p2 ≡ iProto_le_pre iProto_le p1 p2.
+  Proof. apply: (fixpoint_unfold iProto_le_pre'). Qed.
+
   Global Instance iProto_le_ne : NonExpansive2 (@iProto_le Σ V).
   Proof. solve_proper. Qed.
   Global Instance iProto_le_proper : Proper ((≡) ==> (≡) ==> (⊣⊢)) (@iProto_le Σ V).
   Proof. solve_proper. Qed.
-
-  Lemma iProto_le_unfold p1 p2 : iProto_le p1 p2 ≡ iProto_le_pre iProto_le p1 p2.
-  Proof. apply: (fixpoint_unfold iProto_le_pre'). Qed.
-
-  Lemma iProto_le_refl p : ⊢ iProto_le p p.
+  Global Instance iProto_le_is_except_0 p1 p2 : IsExcept0 (p1 ⊑ p2).
   Proof.
-    iLöb as "IH" forall (p). destruct (proto_case p) as [->|([]&pc&->)].
-    - rewrite iProto_le_unfold. iLeft; by auto.
-    - rewrite iProto_le_unfold. iRight. iExists _, _, _, _; do 2 (iSplit; [done|]).
-      iIntros "!>" (v p') "Hpc". iExists p'. iFrame "Hpc". iApply "IH".
-    - rewrite iProto_le_unfold. iRight. iExists _, _, _, _; do 2 (iSplit; [done|]).
-      iIntros "!>" (v p') "Hpc". iExists p'. iFrame "Hpc". iApply "IH".
+    rewrite /IsExcept0 /sbi_except_0. iIntros "[H|$]".
+    rewrite iProto_le_unfold /iProto_le_pre. iLeft. by iMod "H".
   Qed.
 
-  Lemma iProto_le_end_inv p : iProto_le p proto_end -∗ p ≡ proto_end.
+  Lemma iProto_le_end : ⊢ END ⊑ (END : iProto Σ V).
+  Proof. rewrite iProto_le_unfold. iLeft. auto 10. Qed.
+
+  Lemma iProto_le_send m1 m2 :
+    (∀ v p2', m2 v (Next p2') -∗ ◇ ∃ p1', ▷ (p1' ⊑ p2') ∗ m1 v (Next p1')) -∗
+    (<!> m1) ⊑ (<!> m2).
+  Proof. rewrite iProto_le_unfold. iIntros "H". iRight. auto 10. Qed.
+  Lemma iProto_le_recv m1 m2 :
+    (∀ v p1', m1 v (Next p1') -∗ ◇ ∃ p2', ▷ (p1' ⊑ p2') ∗ m2 v (Next p2')) -∗
+    (<?> m1) ⊑ (<?> m2).
+  Proof. rewrite iProto_le_unfold. iIntros "H". iRight. auto 10. Qed.
+  Lemma iProto_le_swap m1 m2 :
+    (∀ v1 v2 p1' p2',
+       m1 v1 (Next p1') -∗ m2 v2 (Next p2') -∗ ◇ ∃ m1' m2' pt,
+         ▷ (p1' ⊑ <!> m1') ∗ ▷ ((<?> m2') ⊑ p2') ∗
+         m1' v2 (Next pt) ∗ m2' v1 (Next pt)) -∗
+    (<?> m1) ⊑ (<!> m2).
+  Proof. rewrite iProto_le_unfold. iIntros "H". iRight. auto 10. Qed.
+
+  Lemma iProto_le_end_inv p : p ⊑ END -∗ ◇ (p ≡ END).
   Proof.
     rewrite iProto_le_unfold. iIntros "[[Hp _]|H] //".
-    iDestruct "H" as (a1 a2 pc1 pc2) "(_ & Heq & _)".
-    by iDestruct (proto_end_message_equivI with "Heq") as %[].
+    iDestruct "H" as (a1 a2 m1 m2) "(_ & >Heq & _)".
+    by iDestruct (iProto_end_message_equivI with "Heq") as %[].
   Qed.
 
-  Lemma iProto_le_send_inv p1 pc2 :
-    iProto_le p1 (proto_message Send pc2) -∗ ∃ a1 pc1,
-      p1 ≡ proto_message a1 pc1 ∗
+  Lemma iProto_le_send_inv p1 m2 :
+    p1 ⊑ (<!> m2) -∗ ∃ a1 m1,
+      ◇ (p1 ≡ <a1> m1) ∗
       match a1 with
-      | Send => ▷ ∀ v p2', pc2 v p2' -∗ ∃ p1', iProto_le p1' p2' ∗ pc1 v p1'
-      | Recv => ▷ ∀ v1 v2 p1' p2',
-         pc1 v1 p1' -∗ pc2 v2 p2' -∗ ∃ pc1' pc2' pt,
-           iProto_le p1' (proto_message Send pc1') ∗
-           iProto_le (proto_message Recv pc2') p2' ∗
-           pc1' v2 pt ∗
-           pc2' v1 pt
+      | Send => ∀ v p2',
+         m2 v (Next p2') -∗ ◇ ∃ p1', ▷ (p1' ⊑ p2') ∗ m1 v (Next p1')
+      | Recv => ∀ v1 v2 p1' p2',
+         m1 v1 (Next p1') -∗ m2 v2 (Next p2') -∗ ◇ ∃ m1' m2' pt,
+           ▷ (p1' ⊑ <!> m1') ∗ ▷ ((<?> m2') ⊑ p2') ∗
+           m1' v2 (Next pt) ∗ m2' v1 (Next pt)
       end.
   Proof.
     rewrite iProto_le_unfold. iIntros "[[_ Heq]|H]".
-    { by iDestruct (proto_message_end_equivI with "Heq") as %[]. }
-    iDestruct "H" as (a1 a2 pc1 pc2') "(Hp1 & Hp2 & H)".
-    iDestruct (proto_message_equivI with "Hp2") as (<-) "{Hp2} #Hpc".
-    iExists _, _; iSplit; [done|]. destruct a1.
-    - iIntros "!>" (v p2'). by iRewrite ("Hpc" $! v p2').
-    - iIntros "!>" (v1 v2 p1' p2'). by iRewrite ("Hpc" $! v2 p2').
+    { iExists inhabitant, inhabitant.
+      iSplit; [|destruct inhabitant];
+        iMod "Heq"; iDestruct (iProto_message_end_equivI with "Heq") as %[]. }
+    iDestruct "H" as (a1 a2 m1 m2') "(Hp1 & Hp2 & H)".
+    iExists _, _; iSplit; [done|]. destruct a1, a2.
+    - iIntros (v p2') "Hm2". iMod "Hp1". iMod "Hp2".
+      iDestruct (iProto_message_equivI with "Hp2") as (_) "{Hp2} #Hm".
+      iApply "H". by iRewrite -("Hm" $! v (Next p2')).
+    - done.
+    - iIntros (v1 v2 p1' p2') "Hm1 Hm2". iMod "Hp1". iMod "Hp2".
+      iDestruct (iProto_message_equivI with "Hp2") as (_) "{Hp2} #Hm".
+      iApply ("H" with "Hm1"). by iRewrite -("Hm" $! v2 (Next p2')).
+    - iMod "Hp2". iDestruct (iProto_message_equivI with "Hp2") as ([=]) "_".
+  Qed.
+  Lemma iProto_le_send_send_inv m1 m2 v p2' :
+    (<!> m1) ⊑ (<!> m2) -∗
+    m2 v (Next p2') -∗ ◇ ∃ p1', ▷ (p1' ⊑ p2') ∗ m1 v (Next p1').
+  Proof.
+    iIntros "H Hm2". iDestruct (iProto_le_send_inv with "H") as (a m1') "[>Hm1 H]".
+    iDestruct (iProto_message_equivI with "Hm1") as (<-) "Hm1".
+    iMod ("H" with "Hm2") as (p1') "[Hle Hm]".
+    iRewrite -("Hm1" $! v (Next p1')) in "Hm". auto with iFrame.
+  Qed.
+  Lemma iProto_le_recv_send_inv m1 m2 v1 v2 p1' p2' :
+    (<?> m1) ⊑ (<!> m2) -∗
+    m1 v1 (Next p1') -∗ m2 v2 (Next p2') -∗ ◇ ∃ m1' m2' pt,
+      ▷ (p1' ⊑ <!> m1') ∗ ▷ ((<?> m2') ⊑ p2') ∗
+      m1' v2 (Next pt) ∗ m2' v1 (Next pt).
+  Proof.
+    iIntros "H Hm1 Hm2". iDestruct (iProto_le_send_inv with "H") as (a m1') "[>Hm H]".
+    iDestruct (iProto_message_equivI with "Hm") as (<-) "{Hm} #Hm".
+    iApply ("H" with "[Hm1] Hm2"). by iRewrite -("Hm" $! v1 (Next p1')).
   Qed.
 
-  Lemma iProto_le_recv_inv p1 pc2 :
-    iProto_le p1 (proto_message Recv pc2) -∗ ∃ pc1,
-      p1 ≡ proto_message Recv pc1 ∗
-      ▷ ∀ v p1', pc1 v p1' -∗ ∃ p2', iProto_le p1' p2' ∗ pc2 v p2'.
+  Lemma iProto_le_recv_inv p1 m2 :
+    p1 ⊑ (<?> m2) -∗ ∃ m1,
+      ◇ (p1 ≡ <?> m1) ∗
+      ∀ v p1', m1 v (Next p1') -∗ ◇ ∃ p2', ▷ (p1' ⊑ p2') ∗ m2 v (Next p2').
   Proof.
     rewrite iProto_le_unfold. iIntros "[[_ Heq]|H]".
-    { by iDestruct (proto_message_end_equivI with "Heq") as %[]. }
-    iDestruct "H" as (a1 a2 pc1 pc2') "(Hp1 & Hp2 & H)".
-    iDestruct (proto_message_equivI with "Hp2") as (<-) "{Hp2} #Hpc2".
-    destruct a1; [done|]. iExists _; iSplit; [done|].
-    iIntros "!>" (v p1') "Hpc". iDestruct ("H" with "Hpc") as (p2') "[Hle Hpc]".
-    iExists p2'. iFrame "Hle". by iRewrite ("Hpc2" $! v p2').
+    { iExists inhabitant.
+      iSplit; iMod "Heq"; iDestruct (iProto_message_end_equivI with "Heq") as %[]. }
+    iDestruct "H" as (a1 a2 m1 m2') "(Hp1 & Hp2 & H)".
+    iExists m1. iSplit; iMod "Hp1"; iMod "Hp2";
+      iDestruct (iProto_message_equivI with "Hp2") as (<-) "{Hp2} #Hm2";
+      destruct a1; try done.
+    iIntros (v p1') "Hm". iMod ("H" with "Hm") as (p2') "[Hle Hm]".
+    iExists p2'. iIntros "{$Hle}". by iRewrite ("Hm2" $! v (Next p2')).
+  Qed.
+  Lemma iProto_le_recv_recv_inv m1 m2 v p1' :
+    (<?> m1) ⊑ (<?> m2) -∗
+    m1 v (Next p1') -∗ ◇ ∃ p2', ▷ (p1' ⊑ p2') ∗ m2 v (Next p2').
+  Proof.
+    iIntros "H Hm2". iDestruct (iProto_le_recv_inv with "H") as (m1') "[>Hm1 H]".
+    iApply "H". iDestruct (iProto_message_equivI with "Hm1") as (_) "Hm1".
+    by iRewrite -("Hm1" $! v (Next p1')).
   Qed.
 
-  Lemma iProto_le_trans p1 p2 p3 :
-    iProto_le p1 p2 -∗ iProto_le p2 p3 -∗ iProto_le p1 p3.
+  Lemma iProto_le_refl p : ⊢ p ⊑ p.
+  Proof.
+    iLöb as "IH" forall (p). destruct (iProto_case p) as [->|([]&m&->)].
+    - iApply iProto_le_end.
+    - iApply iProto_le_send. auto 10 with iFrame.
+    - iApply iProto_le_recv. auto 10 with iFrame.
+  Qed.
+
+  Lemma iProto_le_trans p1 p2 p3 : p1 ⊑ p2 -∗ p2 ⊑ p3 -∗ p1 ⊑ p3.
   Proof.
     iIntros "H1 H2". iLöb as "IH" forall (p1 p2 p3).
-    destruct (proto_case p3) as [->|([]&pc3&->)].
-    - by iRewrite (iProto_le_end_inv with "H2") in "H1".
-    - iDestruct (iProto_le_send_inv with "H2") as (a2 pc2) "[Hp2 H2]".
+    destruct (iProto_case p3) as [->|([]&m3&->)].
+    - iMod (iProto_le_end_inv with "H2") as "H2". by iRewrite "H2" in "H1".
+    - iDestruct (iProto_le_send_inv with "H2") as (a2 m2) "[>Hp2 H2]".
       iRewrite "Hp2" in "H1"; clear p2. destruct a2.
-      + iDestruct (iProto_le_send_inv with "H1") as (a1 pc1) "[Hp1 H1]".
-        iRewrite "Hp1"; clear p1. rewrite iProto_le_unfold; iRight.
-        iExists _, _, _, _; do 2 (iSplit; [done|]). destruct a1.
-        * iIntros "!>" (v p3') "Hpc".
-          iDestruct ("H2" with "Hpc") as (p2') "[Hle Hpc]".
-          iDestruct ("H1" with "Hpc") as (p1') "[Hle' Hpc]".
-          iExists p1'. iFrame "Hpc". by iApply ("IH" with "Hle'").
-        * iIntros "!>" (v1 v3 p1' p3') "Hpc1 Hpc3".
-          iDestruct ("H2" with "Hpc3") as (p2') "[Hle Hpc2]".
-          iDestruct ("H1" with "Hpc1 Hpc2") as (pc1' pc2' pt) "(Hp1' & Hp2' & Hpc)".
-          iExists pc1', pc2', pt. iFrame "Hp1' Hpc". by iApply ("IH" with "Hp2'").
-      + iDestruct (iProto_le_recv_inv with "H1") as (pc1) "[Hp1 H1]".
-        iRewrite "Hp1"; clear p1. rewrite iProto_le_unfold; iRight.
-        iExists _, _, _, _; do 2 (iSplit; [done|]); simpl.
-        iIntros "!>" (v1 v3 p1' p3') "Hpc1 Hpc3".
-        iDestruct ("H1" with "Hpc1") as (p2') "[Hle Hpc2]".
-        iDestruct ("H2" with "Hpc2 Hpc3") as (pc2' pc3' pt) "(Hp2' & Hp3' & Hpc)".
-        iExists pc2', pc3', pt. iFrame "Hp3' Hpc". by iApply ("IH" with "Hle").
-    - iDestruct (iProto_le_recv_inv with "H2") as (pc2) "[Hp2 H3]".
+      + iDestruct (iProto_le_send_inv with "H1") as (a1 m1) "[>Hp1 H1]".
+        iRewrite "Hp1"; clear p1. destruct a1.
+        * iApply iProto_le_send. iIntros (v p3') "Hm3".
+          iMod ("H2" with "Hm3") as (p2') "[Hle Hm2]".
+          iMod ("H1" with "Hm2") as (p1') "[Hle' Hm1]".
+          iExists p1'. iIntros "{$Hm1} !>". by iApply ("IH" with "Hle'").
+        * iApply iProto_le_swap. iIntros (v1 v3 p1' p3') "Hm1 Hm3".
+          iMod ("H2" with "Hm3") as (p2') "[Hle Hm2]".
+          iMod ("H1" with "Hm1 Hm2") as (m1' m2' pt) "(Hp1' & Hp2' & Hm)".
+          iExists m1', m2', pt. iIntros "{$Hp1' $Hm} !>". by iApply ("IH" with "Hp2'").
+      + iDestruct (iProto_le_recv_inv with "H1") as (m1) "[>Hp1 H1]".
+        iRewrite "Hp1"; clear p1. iApply iProto_le_swap.
+        iIntros (v1 v3 p1' p3') "Hm1 Hm3".
+        iMod ("H1" with "Hm1") as (p2') "[Hle Hm2]".
+        iMod ("H2" with "Hm2 Hm3") as (m2' m3' pt) "(Hp2' & Hp3' & Hm)".
+        iExists m2', m3', pt. iIntros "{$Hp3' $Hm} !>". by iApply ("IH" with "Hle").
+    - iDestruct (iProto_le_recv_inv with "H2") as (m2) "[>Hp2 H3]".
       iRewrite "Hp2" in "H1".
-      iDestruct (iProto_le_recv_inv with "H1") as (pc1) "[Hp1 H2]".
-      iRewrite "Hp1". rewrite iProto_le_unfold. iRight.
-      iExists _, _, _, _; do 2 (iSplit; [done|]).
-      iIntros "!>" (v p1') "Hpc".
-      iDestruct ("H2" with "Hpc") as (p2') "[Hle Hpc]".
-      iDestruct ("H3" with "Hpc") as (p3') "[Hle' Hpc]".
-      iExists p3'. iFrame "Hpc". by iApply ("IH" with "Hle").
+      iDestruct (iProto_le_recv_inv with "H1") as (m1) "[>Hp1 H2]".
+      iRewrite "Hp1". iApply iProto_le_recv. iIntros (v p1') "Hm1".
+      iMod ("H2" with "Hm1") as (p2') "[Hle Hm2]".
+      iMod ("H3" with "Hm2") as (p3') "[Hle' Hm3]".
+      iExists p3'. iIntros "{$Hm3} !>". by iApply ("IH" with "Hle").
   Qed.
 
-  Lemma iProto_le_send {TT1 TT2} (pc1 : TT1 → V * iProp Σ * iProto Σ V)
-      (pc2 : TT2 → V * iProp Σ * iProto Σ V) :
-    ▷ (∀.. x2 : TT2, (pc2 x2).1.2 -∗ ∃.. x1 : TT1,
-      ⌜(pc1 x1).1.1 = (pc2 x2).1.1⌝ ∗
-      (pc1 x1).1.2 ∗
-      iProto_le (pc1 x1).2 (pc2 x2).2) -∗
-    iProto_le (iProto_message Send pc1) (iProto_message Send pc2).
+  Lemma iProto_le_base a v P p1 p2 :
+    ▷ (p1 ⊑ p2) -∗
+    (<a> MSG v {{ P }}; p1) ⊑ (<a> MSG v {{ P }}; p2).
   Proof.
-    iIntros "H". rewrite iProto_le_unfold iProto_message_eq.
-    iRight. iExists _, _, _, _; do 2 (iSplit; [done|]).
-    iIntros "!>" (v p2') "/=". iDestruct 1 as (x2 ->) "[Hpc #Heq]".
-    iDestruct ("H" with "Hpc") as (x1 ?) "[Hpc Hle]".
-    iExists (pc1 x1).2. iSplitL "Hle"; [by iRewrite "Heq"|].
-    iExists x1. iSplit; [done|]. iSplit; [by iApply "Hpc"|done].
+    rewrite iMsg_base_eq. iIntros "H". destruct a.
+    - iApply iProto_le_send. iIntros (v' p') "(->&Hp&$) !>".
+      iExists p1. iSplit; [|by auto]. iIntros "!>". by iRewrite -"Hp".
+    - iApply iProto_le_recv. iIntros (v' p') "(->&Hp&$) !>".
+      iExists p2. iSplit; [|by auto]. iIntros "!>". by iRewrite -"Hp".
   Qed.
-
-  Lemma iProto_le_recv {TT1 TT2} (pc1 : TT1 → V * iProp Σ * iProto Σ V)
-      (pc2 : TT2 → V * iProp Σ * iProto Σ V) :
-    ▷ (∀.. x1 : TT1, (pc1 x1).1.2 -∗ ∃.. x2 : TT2,
-      ⌜(pc1 x1).1.1 = (pc2 x2).1.1⌝ ∗
-      (pc2 x2).1.2 ∗
-      iProto_le (pc1 x1).2 (pc2 x2).2) -∗
-    iProto_le (iProto_message Recv pc1) (iProto_message Recv pc2).
+  Lemma iProto_le_base_swap v1 v2 P1 P2 p :
+    ⊢ (<?> MSG v1 {{ P1 }}; <!> MSG v2 {{ P2 }}; p)
+    ⊑ (<!> MSG v2 {{ P2 }}; <?> MSG v1 {{ P1 }}; p).
   Proof.
-    iIntros "H". rewrite iProto_le_unfold iProto_message_eq.
-    iRight. iExists _, _, _, _; do 2 (iSplit; [done|]).
-    iIntros "!>" (v p1') "/=". iDestruct 1 as (x1 ->) "[Hpc #Heq]".
-    iDestruct ("H" with "Hpc") as (x2 ?) "[Hpc Hle]".
-    iExists (pc2 x2).2. iSplitL "Hle"; [by iRewrite "Heq"|].
-    iExists x2. iSplit; [done|]. iSplit; [by iApply "Hpc"|done].
+    rewrite iMsg_base_eq. iApply iProto_le_swap.
+    iIntros (v1' v2' p1' p2') "/= (->&#Hp1&HP1) (->&#Hp2&HP2) !>". iExists _, _, p.
+    iSplitR; [iIntros "!>"; iRewrite -"Hp1"; iApply iProto_le_refl|].
+    iSplitR; [iIntros "!>"; iRewrite -"Hp2"; iApply iProto_le_refl|].
+    simpl; auto with iFrame.
   Qed.
 
-  Lemma iProto_le_swap {TT1 TT2} (pc1 : TT1 → V * iProp Σ * iProto Σ V)
-      (pc2 : TT2 → V * iProp Σ * iProto Σ V) :
-    ▷ (∀.. (x1 : TT1) (x2 : TT2),
-      (pc1 x1).1.2 -∗ (pc2 x2).1.2 -∗
-      ∃ {TT3 TT4} (pc3 : TT3 → V * iProp Σ * iProto Σ V)
-          (pc4 : TT4 → V * iProp Σ * iProto Σ V), ∃.. (x3 : TT3) (x4 : TT4),
-        ⌜(pc1 x1).1.1 = (pc4 x4).1.1⌝ ∗
-        ⌜(pc2 x2).1.1 = (pc3 x3).1.1⌝ ∗
-        iProto_le (pc1 x1).2 (iProto_message Send pc3) ∗
-        iProto_le (iProto_message Recv pc4) (pc2 x2).2 ∗
-        (pc3 x3).1.2 ∗ (pc4 x4).1.2 ∗
-        ((pc3 x3).2 ≡ (pc4 x4).2)) -∗
-    iProto_le (iProto_message Recv pc1) (iProto_message Send pc2).
+  Lemma iProto_le_payload_elim_l a m v P p :
+    (P -∗ (<?> MSG v; p) ⊑ (<a> m)) -∗
+    (<?> MSG v {{ P }}; p) ⊑ (<a> m).
   Proof.
-    iIntros "H". rewrite iProto_le_unfold iProto_message_eq.
-    iRight. iExists _, _, _, _; do 2 (iSplit; [done|]); simpl.
-    iIntros "!>" (v1 v2 p1 p2).
-    iDestruct 1 as (x1 ->) "[Hpc1 #Heq1]"; iDestruct 1 as (x2 ->) "[Hpc2 #Heq2]".
-    iDestruct ("H" with "Hpc1 Hpc2")
-      as (TT3 TT4 pc3 pc4 x3 x4 ??) "(H1 & H2 & Hpc1 & Hpc2 & #H)".
-    iExists _, _, (pc3 x3).2. iSplitL "H1"; [by iRewrite "Heq1"|].
-    iSplitL "H2"; [by iRewrite "Heq2"|]. simpl. iSplitL "Hpc1"; eauto.
+    rewrite iMsg_base_eq. iIntros "H". destruct a.
+    - iApply iProto_le_swap. iIntros (v1 v2 p1' p2') "/= (#?&#?&HP) Hm2 /=".
+      iApply (iProto_le_recv_send_inv with "(H HP)"); simpl; auto.
+    - iApply iProto_le_recv. iIntros (v' p') "(->&Hp&HP)".
+      iApply (iProto_le_recv_recv_inv with "(H HP)"); simpl; auto.
   Qed.
-
-  Lemma iProto_le_swap_simple {TT1 TT2} (v1 : TT1 → V) (v2 : TT2 → V)
-      (P1 : TT1 → iProp Σ) (P2 : TT2 → iProp Σ) (p : TT1 → TT2 → iProto Σ V) :
-    ⊢ iProto_le
-        (iProto_message Recv (λ x1,
-          (v1 x1, P1 x1, iProto_message Send (λ x2, (v2 x2, P2 x2, p x1 x2)))))
-        (iProto_message Send (λ x2,
-          (v2 x2, P2 x2, iProto_message Recv (λ x1, (v1 x1, P1 x1, p x1 x2))))).
+  Lemma iProto_le_payload_elim_r a m v P p :
+    (P -∗ (<a> m) ⊑ (<!> MSG v; p)) -∗
+    (<a> m) ⊑ (<!> MSG v {{ P }}; p).
   Proof.
-    iApply iProto_le_swap. iIntros "!>" (x1 x2) "/= HP1 HP2".
-    iExists TT2, TT1, (λ x2, (v2 x2, P2 x2, p x1 x2)),
-      (λ x1, (v1 x1, P1 x1, p x1 x2)), x2, x1; simpl.
-    do 2 (iSplit; [done|]). do 2 (iSplitR; [iApply iProto_le_refl|]). by iFrame.
+    rewrite iMsg_base_eq. iIntros "H". destruct a.
+    - iApply iProto_le_send. iIntros (v' p') "(->&Hp&HP)".
+      iApply (iProto_le_send_send_inv with "(H HP)"); simpl; auto.
+    - iApply iProto_le_swap. iIntros (v1 v2 p1' p2') "/= Hm1 (->&#?&HP) /=".
+      iApply (iProto_le_recv_send_inv with "(H HP) Hm1"); simpl; auto.
+  Qed.
+  Lemma iProto_le_payload_intro_l v P p :
+    P -∗ (<!> MSG v {{ P }}; p) ⊑ (<!> MSG v; p).
+  Proof.
+    rewrite iMsg_base_eq.
+    iIntros "HP". iApply iProto_le_send. iIntros (v' p') "(->&Hp&_) !> /=".
+    iExists p'. iSplitR; [iApply iProto_le_refl|]. auto.
+  Qed.
+  Lemma iProto_le_payload_intro_r v P p :
+    P -∗ (<?> MSG v; p) ⊑ (<?> MSG v {{ P }}; p).
+  Proof.
+    rewrite iMsg_base_eq.
+    iIntros "HP". iApply iProto_le_recv. iIntros (v' p') "(->&Hp&_) !> /=".
+    iExists p'. iSplitR; [iApply iProto_le_refl|]. auto.
   Qed.
 
-  Lemma iProto_le_dual p1 p2 :
-    iProto_le p2 p1 -∗ iProto_le (iProto_dual p1) (iProto_dual p2).
+  Lemma iProto_le_exist_elim_l {A} (m1 : A → iMsg Σ V) a m2 :
+    (∀ x, (<?> m1 x) ⊑ (<a> m2)) -∗
+    (<? x> m1 x) ⊑ (<a> m2).
+  Proof.
+    rewrite iMsg_exist_eq. iIntros "H". destruct a.
+    - iApply iProto_le_swap. iIntros (v1 v2 p1' p2') "/= Hm1 Hm2 /=".
+      iDestruct "Hm1" as (x) "Hm1".
+      iApply (iProto_le_recv_send_inv with "H Hm1 Hm2").
+    - iApply iProto_le_recv. iIntros (v p1') "/=". iDestruct 1 as (x) "Hm".
+      by iApply (iProto_le_recv_recv_inv with "H").
+  Qed.
+  Lemma iProto_le_exist_elim_r {A} a m1 (m2 : A → iMsg Σ V) :
+    (∀ x, (<a> m1) ⊑ (<!> m2 x)) -∗
+    (<a> m1) ⊑ (<! x> m2 x).
+  Proof.
+    rewrite iMsg_exist_eq. iIntros "H". destruct a.
+    - iApply iProto_le_send. iIntros (v p2'). iDestruct 1 as (x) "Hm".
+      by iApply (iProto_le_send_send_inv with "H").
+    - iApply iProto_le_swap. iIntros (v1 v2 p1' p2') "/= Hm1".
+      iDestruct 1 as (x) "Hm2".
+      iApply (iProto_le_recv_send_inv with "H Hm1 Hm2").
+  Qed.
+  Lemma iProto_le_exist_intro_l {A} (m : A → iMsg Σ V) a :
+    ⊢ (<! x> m x) ⊑ (<!> m a).
+  Proof.
+    rewrite iMsg_exist_eq. iApply iProto_le_send. iIntros (v p') "Hm !> /=".
+    iExists p'. iSplitR; last by auto. iApply iProto_le_refl.
+  Qed.
+  Lemma iProto_le_exist_intro_r {A} (m : A → iMsg Σ V) a :
+    ⊢ (<?> m a) ⊑ (<? x> m x).
+  Proof.
+    rewrite iMsg_exist_eq. iApply iProto_le_recv. iIntros (v p') "Hm !> /=".
+    iExists p'. iSplitR; last by auto. iApply iProto_le_refl.
+  Qed.
+
+  Lemma iProto_le_texist_elim_l {TT : tele} (m1 : TT → iMsg Σ V) a m2 :
+    (∀ x, (<?> m1 x) ⊑ (<a> m2)) -∗
+    (<?.. x> m1 x) ⊑ (<a> m2).
+  Proof.
+    iIntros "H". iInduction TT as [|T TT] "IH"; simpl; [done|].
+    iApply iProto_le_exist_elim_l; iIntros (x).
+    iApply "IH". iIntros (xs). iApply "H".
+  Qed.
+  Lemma iProto_le_texist_elim_r {TT : tele} a m1 (m2 : TT → iMsg Σ V) :
+    (∀ x, (<a> m1) ⊑ (<!> m2 x)) -∗
+    (<a> m1) ⊑ (<!.. x> m2 x).
+  Proof.
+    iIntros "H". iInduction TT as [|T TT] "IH"; simpl; [done|].
+    iApply iProto_le_exist_elim_r; iIntros (x).
+    iApply "IH". iIntros (xs). iApply "H".
+  Qed.
+  Lemma iProto_le_texist_intro_l {TT : tele} (m : TT → iMsg Σ V) x :
+    ⊢ (<!.. x> m x) ⊑ (<!> m x).
+  Proof.
+    induction x as [|T TT x xs IH]; simpl; [iApply iProto_le_refl|].
+    iApply iProto_le_trans; [by iApply iProto_le_exist_intro_l|]. iApply IH.
+  Qed.
+  Lemma iProto_le_texist_intro_r {TT : tele} (m : TT → iMsg Σ V) x :
+    ⊢ (<?> m x) ⊑ (<?.. x> m x).
+  Proof.
+    induction x as [|T TT x xs IH]; simpl; [iApply iProto_le_refl|].
+    iApply iProto_le_trans; [|by iApply iProto_le_exist_intro_r]. iApply IH.
+  Qed.
+
+  Lemma iProto_le_dual p1 p2 : p2 ⊑ p1 -∗ iProto_dual p1 ⊑ iProto_dual p2.
   Proof.
     iIntros "H". iLöb as "IH" forall (p1 p2).
-    destruct (proto_case p1) as [->|([]&pc1&->)].
-    - iRewrite (iProto_le_end_inv with "H"). iApply iProto_le_refl.
-    - iDestruct (iProto_le_send_inv with "H") as (a2 pc2) "[Hp2 H]".
-      iRewrite "Hp2"; clear p2. iEval (rewrite !iProto_dual_message').
-      rewrite iProto_le_unfold; iRight.
-      iExists _, _, _, _; do 2 (iSplit; [done|]); simpl. destruct a2; simpl.
-      + iIntros "!>" (v p1d). iDestruct 1 as (p1') "[Hpc #Hp1d]".
-        iDestruct ("H" with "Hpc") as (p2') "[H Hpc]".
-        iDestruct ("IH" with "H") as "H".
-        iExists (iProto_dual p2'). iSplitR "Hpc"; [|by auto]. by iRewrite "Hp1d".
-      + iIntros "!>" (v1 v2 p1d p2d).
-        iDestruct 1 as (p1') "[Hpc1 #Hp1d]". iDestruct 1 as (p2') "[Hpc2 #Hp2d]".
-        iDestruct ("H" with "Hpc2 Hpc1") as (pc1' pc2' pt) "(H1 & H2 & Hpc1 & Hpc2)".
+    destruct (iProto_case p1) as [->|([]&m1&->)].
+    - iMod (iProto_le_end_inv with "H") as "H".
+      iRewrite "H". iApply iProto_le_refl.
+    - iDestruct (iProto_le_send_inv with "H") as (a2 m2) "[>Hp2 H]".
+      iRewrite "Hp2"; clear p2. iEval (rewrite !iProto_dual_message).
+      destruct a2; simpl.
+      + iApply iProto_le_recv. iIntros (v p1d).
+        iDestruct 1 as (p1') "[Hm1 #Hp1d]".
+        iMod ("H" with "Hm1") as (p2') "[H Hm2]".
+        iDestruct ("IH" with "H") as "H". iIntros "!>". iExists (iProto_dual p2').
+        iSplitL "H"; [iIntros "!>"; by iRewrite "Hp1d"|]. simpl; auto.
+      + iApply iProto_le_swap. iIntros (v1 p1d v2 p2d).
+        iDestruct 1 as (p1') "[Hm1 #Hp1d]". iDestruct 1 as (p2') "[Hm2 #Hp2d]".
+        iMod ("H" with "Hm2 Hm1") as (m1' m2' pt) "(H1 & H2 & Hm1 & Hm2)".
         iDestruct ("IH" with "H1") as "H1". iDestruct ("IH" with "H2") as "H2 {IH}".
-        rewrite !iProto_dual_message' /=. iExists _, _, (iProto_dual pt).
-        iSplitL "H2"; [by iRewrite "Hp1d"|]. iSplitL "H1"; [by iRewrite "Hp2d"|].
-        iSplitL "Hpc2"; simpl; auto.
-    - iDestruct (iProto_le_recv_inv with "H") as (pc2) "[Hp2 H]".
-      iRewrite "Hp2"; clear p2. iEval (rewrite !iProto_dual_message' /=).
-      rewrite iProto_le_unfold; iRight.
-      iExists _, _, _, _; do 2 (iSplit; [done|]); simpl.
-      iIntros "!>" (v p2d). iDestruct 1 as (p2') "[Hpc #Hp2d]".
-      iDestruct ("H" with "Hpc") as (p1') "[H Hpc]".
-      iDestruct ("IH" with "H") as "H".
-      iExists (iProto_dual p1'). iSplitR "Hpc"; [|by auto]. by iRewrite "Hp2d".
+        rewrite !iProto_dual_message /=. iIntros "!>". iExists _, _, (iProto_dual pt).
+        iSplitL "H2"; [iIntros "!>"; by iRewrite "Hp1d"|].
+        iSplitL "H1"; [iIntros "!>"; by iRewrite "Hp2d"|].
+        iSplitL "Hm2"; simpl; auto.
+    - iDestruct (iProto_le_recv_inv with "H") as (m2) "[>Hp2 H]".
+      iRewrite "Hp2"; clear p2. iEval (rewrite !iProto_dual_message /=).
+      iApply iProto_le_send. iIntros (v p2d).
+      iDestruct 1 as (p2') "[Hm2 #Hp2d]".
+      iMod ("H" with "Hm2") as (p1') "[H Hm1]".
+      iDestruct ("IH" with "H") as "H". iIntros "!>". iExists (iProto_dual p1').
+      iSplitL "H"; [iIntros "!>"; by iRewrite "Hp2d"|]. simpl; auto.
   Qed.
 
-  Lemma iProto_le_dual_l p1 p2 :
-    iProto_le (iProto_dual p2) p1 -∗ iProto_le (iProto_dual p1) p2.
+  Lemma iProto_le_dual_l p1 p2 : iProto_dual p2 ⊑ p1 -∗ iProto_dual p1 ⊑ p2.
   Proof.
     iIntros "H". iEval (rewrite -(involutive iProto_dual p2)).
     by iApply iProto_le_dual.
   Qed.
-  Lemma iProto_le_dual_r p1 p2 :
-    iProto_le p2 (iProto_dual p1) -∗ iProto_le p1 (iProto_dual p2).
+  Lemma iProto_le_dual_r p1 p2 : p2 ⊑ iProto_dual p1 -∗ p1 ⊑ iProto_dual p2.
   Proof.
     iIntros "H". iEval (rewrite -(involutive iProto_dual p1)).
     by iApply iProto_le_dual.
   Qed.
 
   Lemma iProto_le_app p1 p2 p3 p4 :
-    iProto_le p1 p2 -∗ iProto_le p3 p4 -∗ iProto_le (p1 <++> p3) (p2 <++> p4).
+    p1 ⊑ p2 -∗ p3 ⊑ p4 -∗ p1 <++> p3 ⊑ p2 <++> p4.
   Proof.
     iIntros "H1 H2". iLöb as "IH" forall (p1 p2 p3 p4).
-    destruct (proto_case p2) as [->|([]&pc2&->)].
-    - iRewrite (iProto_le_end_inv with "H1"). by rewrite !iProto_app_end'.
-    - iDestruct (iProto_le_send_inv with "H1") as (a1 pc1) "[Hp1 H1]".
-      iRewrite "Hp1"; clear p1.
-      rewrite !iProto_app_message'. iEval (rewrite iProto_le_unfold).
-      iRight. iExists _, _, _, _; do 2 (iSplit; [done|]). destruct a1; simpl.
-      + iIntros "!>" (v p24). iDestruct 1 as (p2') "[Hpc #Hp24]".
-        iDestruct ("H1" with "Hpc") as (p1') "[H1 Hpc]".
-        iExists (p1' <++> p3)%proto. iSplitR "Hpc"; [|eauto].
-        iRewrite "Hp24". by iApply ("IH" with "H1").
-      + iIntros "!>" (v1 v2 p13 p24).
-        iDestruct 1 as (p1') "[Hpc1 #Hp13]"; iDestruct 1 as (p2') "[Hpc2 #Hp24]".
-        iDestruct ("H1" with "Hpc1 Hpc2") as (pc1' pc2' pt) "(H1 & H1' & Hpc1 & Hpc2)".
-        iExists (iProto_map_app_cont (flip iProto_app p3) ∘ pc1'),
-          (iProto_map_app_cont (flip iProto_app p3) ∘ pc2'), (pt <++> p3)%proto.
-        rewrite -!iProto_app_message' /=. iSplitL "H1".
-        { iRewrite "Hp13". iApply ("IH" with "H1"). iApply iProto_le_refl. }
+    destruct (iProto_case p2) as [->|([]&m2&->)].
+    - iMod (iProto_le_end_inv with "H1") as "H1".
+      iRewrite "H1". by rewrite !left_id.
+    - iDestruct (iProto_le_send_inv with "H1") as (a1 m1) "[>Hp1 H1]".
+      iRewrite "Hp1"; clear p1. rewrite !iProto_app_message. destruct a1; simpl.
+      + iApply iProto_le_send. iIntros (v p24).
+        iDestruct 1 as (p2') "[Hm2 #Hp24]".
+        iMod ("H1" with "Hm2") as (p1') "[H1 Hm1]".
+        iIntros "!>". iExists (p1' <++> p3). iSplitR "Hm1"; [|by simpl; eauto].
+        iIntros "!>". iRewrite "Hp24". by iApply ("IH" with "H1").
+      + iApply iProto_le_swap. iIntros (v1 v2 p13 p24).
+        iDestruct 1 as (p1') "[Hm1 #Hp13]". iDestruct 1 as (p2') "[Hm2 #Hp24]".
+        iSpecialize ("H1" with "Hm1 Hm2").
+        iMod "H1" as (m1' m2' pt) "(H1 & H1' & Hm1 & Hm2)".
+        iIntros "!>". iExists (m1' <++> p3)%msg, (m2' <++> p3)%msg, (pt <++> p3).
+        rewrite -!iProto_app_message /=. iSplitL "H1".
+        { iIntros "!>". iRewrite "Hp13". iApply ("IH" with "H1"). iApply iProto_le_refl. }
         iSplitL "H2 H1'".
-        { iRewrite "Hp24". iApply ("IH" with "H1' H2"). }
-        iSplitL "Hpc1"; auto.
-    - iDestruct (iProto_le_recv_inv with "H1") as (pc1) "[Hp1 H1]".
-      iRewrite "Hp1"; clear p1.
-      rewrite !iProto_app_message'. iEval (rewrite iProto_le_unfold).
-      iRight. iExists _, _, _, _; do 2 (iSplit; [done|]); simpl.
-      iIntros "!>" (v p13). iDestruct 1 as (p1') "[Hpc #Hp13]".
-      iDestruct ("H1" with "Hpc") as (p2'') "[H1 Hpc]".
-      iExists (p2'' <++> p4)%proto. iSplitR "Hpc"; [|eauto].
-      iRewrite "Hp13". by iApply ("IH" with "H1").
+        { iIntros "!>". iRewrite "Hp24". iApply ("IH" with "H1' H2"). }
+        iSplitL "Hm1"; auto.
+    - iDestruct (iProto_le_recv_inv with "H1") as (m1) "[>Hp1 H1]".
+      iRewrite "Hp1"; clear p1. rewrite !iProto_app_message. iApply iProto_le_recv.
+      iIntros (v p13). iDestruct 1 as (p1') "[Hm1 #Hp13]".
+      iMod ("H1" with "Hm1") as (p2'') "[H1 Hm2]".
+      iIntros "!>". iExists (p2'' <++> p4). iSplitR "Hm2"; [|by simpl; eauto].
+      iIntros "!>". iRewrite "Hp13". by iApply ("IH" with "H1").
   Qed.
 
   (** ** Lemmas about the auxiliary definitions and invariants *)
@@ -797,7 +911,7 @@ Section proto.
     rewrite /iProto_unfold. assert (∀ p, proto_map iProp_unfold iProp_fold
         (proto_map iProp_fold iProp_unfold p) ≡ p) as help.
     { intros p''. rewrite -proto_map_compose -{2}(proto_map_id p'').
-      apply proto_map_ext=> // pc /=; by rewrite iProp_fold_unfold. }
+      apply proto_map_ext=> // m /=; by rewrite iProp_fold_unfold. }
     rewrite -{2}(help p). iRewrite "H✓". by rewrite help.
   Qed.
 
@@ -824,17 +938,17 @@ Section proto.
       (∃ p,
         ⌜ vsl = [] ⌝ ∗
         ⌜ vsr = [] ⌝ ∗
-        iProto_le p pl ∗
-        iProto_le (iProto_dual p) pr) ∨
-      (∃ vl vsl' pc pr',
+        p ⊑ pl ∗
+        iProto_dual p ⊑ pr) ∨
+      (∃ vl vsl' m pr',
         ⌜ vsl = vl :: vsl' ⌝ ∗
-        iProto_le (proto_message Recv pc) pr ∗
-        pc vl pr' ∗
+        (<?> m) ⊑ pr ∗
+        m vl (Next pr') ∗
         iProto_interp vsl' vsr pl pr') ∨
-      (∃ vr vsr' pc pl',
+      (∃ vr vsr' m pl',
         ⌜ vsr = vr :: vsr' ⌝ ∗
-        iProto_le (proto_message Recv pc) pl ∗
-        pc vr pl' ∗
+        (<?> m) ⊑ pl ∗
+        m vr (Next pl') ∗
         iProto_interp vsl vsr' pl' pr).
   Proof.
     rewrite {1}/iProto_interp. destruct vsl as [|vl vsl]; simpl.
@@ -867,16 +981,16 @@ Section proto.
     rewrite !iProto_interp_unfold. iIntros "[H|[H|H]]".
     - iClear "IH". iDestruct "H" as (p -> ->) "[Hp Hp'] /=".
       iLeft. iExists (iProto_dual p). rewrite involutive. iFrame; auto.
-    - iDestruct "H" as (vl vsl' pc' pr' ->) "(Hpr & Hpc' & H)".
-      iRight; iRight. iExists vl, vsl', pc', pr'. iSplit; [done|]; iFrame.
+    - iDestruct "H" as (vl vsl' m' pr' ->) "(Hpr & Hm' & H)".
+      iRight; iRight. iExists vl, vsl', m', pr'. iSplit; [done|]; iFrame.
       iApply ("IH" with "[%] [//] H"); simpl; lia.
-    - iDestruct "H" as (vr vsr' pc' pl' ->) "(Hpl & Hpc' & H)".
-      iRight; iLeft. iExists vr, vsr', pc', pl'. iSplit; [done|]; iFrame.
+    - iDestruct "H" as (vr vsr' m' pl' ->) "(Hpl & Hm' & H)".
+      iRight; iLeft. iExists vr, vsr', m', pl'. iSplit; [done|]; iFrame.
       iApply ("IH" with "[%] [//] H"); simpl; lia.
   Qed.
 
   Lemma iProto_interp_le_l vsl vsr pl pl' pr :
-    iProto_interp vsl vsr pl pr -∗ iProto_le pl pl' -∗ iProto_interp vsl vsr pl' pr.
+    iProto_interp vsl vsr pl pr -∗ pl ⊑ pl' -∗ iProto_interp vsl vsr pl' pr.
   Proof.
     remember (length vsl + length vsr) as n eqn:Hn.
     iInduction (lt_wf n) as [n _] "IH" forall (vsl vsr pl pr Hn); subst.
@@ -884,76 +998,75 @@ Section proto.
     - iClear "IH". iDestruct "H" as (p -> ->) "[Hp Hp'] /=".
       iLeft. iExists p. do 2 (iSplit; [done|]). iFrame "Hp'".
       by iApply (iProto_le_trans with "Hp").
-    - iDestruct "H" as (vl vsl' pc' pr' ->) "(Hpr & Hpc' & H)".
-      iRight; iLeft. iExists vl, vsl', pc', pr'. iSplit; [done|]; iFrame.
+    - iDestruct "H" as (vl vsl' m' pr' ->) "(Hpr & Hm' & H)".
+      iRight; iLeft. iExists vl, vsl', m', pr'. iSplit; [done|]; iFrame.
       iApply ("IH" with "[%] [//] H Hle"); simpl; lia.
-    - iClear "IH". iDestruct "H" as (vr vsr' pc' pl'' ->) "(Hpl & Hpc' & H)".
-      iRight; iRight. iExists vr, vsr', pc', pl''. iSplit; [done|]; iFrame.
+    - iClear "IH". iDestruct "H" as (vr vsr' m' pl'' ->) "(Hpl & Hm' & H)".
+      iRight; iRight. iExists vr, vsr', m', pl''. iSplit; [done|]; iFrame.
       by iApply (iProto_le_trans with "Hpl").
   Qed.
   Lemma iProto_interp_le_r vsl vsr pl pr pr' :
-    iProto_interp vsl vsr pl pr -∗ iProto_le pr pr' -∗ iProto_interp vsl vsr pl pr'.
+    iProto_interp vsl vsr pl pr -∗ pr ⊑ pr' -∗ iProto_interp vsl vsr pl pr'.
   Proof.
     iIntros "H Hle". iApply iProto_interp_flip.
     iApply (iProto_interp_le_l with "[H] Hle"). by iApply iProto_interp_flip.
   Qed.
 
-  Lemma iProto_interp_send vl pcl vsl vsr pl pr pl' :
+  Lemma iProto_interp_send vl ml vsl vsr pl pr pl' :
     iProto_interp vsl vsr pl pr -∗
-    iProto_le pl (proto_message Send pcl) -∗
-    pcl vl pl' -∗
+    pl ⊑ (<!> ml) -∗
+    ml vl (Next pl') -∗
     ▷^(length vsr) iProto_interp (vsl ++ [vl]) vsr pl' pr.
   Proof.
     iIntros "H Hle". iDestruct (iProto_interp_le_l with "H Hle") as "H".
-    clear pl. iIntros "Hpcl". remember (length vsl + length vsr) as n eqn:Hn.
-    iInduction (lt_wf n) as [n _] "IH" forall (pcl vsl vsr pr pl' Hn); subst.
+    clear pl. iIntros "Hml". remember (length vsl + length vsr) as n eqn:Hn.
+    iInduction (lt_wf n) as [n _] "IH" forall (ml vsl vsr pr pl' Hn); subst.
     rewrite {1}iProto_interp_unfold. iDestruct "H" as "[H|[H|H]]".
     - iClear "IH". iDestruct "H" as (p -> ->) "[Hp Hp'] /=".
       iDestruct (iProto_le_dual with "Hp") as "Hp".
       iDestruct (iProto_le_trans with "Hp Hp'") as "Hp".
-      rewrite iProto_dual_message' /=.
+      rewrite iProto_dual_message /=.
       iApply iProto_interp_unfold. iRight; iLeft.
       iExists vl, [], _, (iProto_dual pl'). iSplit; [done|]. iFrame "Hp"; simpl.
       iSplitL; [by auto|]. iApply iProto_interp_nil.
-    - iDestruct "H" as (vl' vsl' pc' pr' ->) "(Hpr & Hpc' & H)".
-      iDestruct ("IH" with "[%] [//] H Hpcl") as "H"; [simpl; lia|].
+    - iDestruct "H" as (vl' vsl' m' pr' ->) "(Hpr & Hm' & H)".
+      iDestruct ("IH" with "[%] [//] H Hml") as "H"; [simpl; lia|].
       iNext. iApply (iProto_interp_le_r with "[-Hpr] Hpr"); clear pr.
       iApply iProto_interp_unfold. iRight; iLeft.
-      iExists vl', (vsl' ++ [vl]), pc', pr'. iFrame.
+      iExists vl', (vsl' ++ [vl]), m', pr'. iFrame.
       iSplit; [done|]. iApply iProto_le_refl.
-    - iDestruct "H" as (vr' vsr' pc' pl'' ->) "(Hle & Hpcl' & H) /=".
-      iDestruct (iProto_le_send_inv with "Hle") as (a pcl') "[Hpc Hle]".
-      iDestruct (proto_message_equivI with "Hpc") as (<-) "Hpc".
-      iIntros "!>". iRewrite ("Hpc" $! vr' pl'') in "Hpcl'"; clear pc'.
-      iDestruct ("Hle" with "Hpcl' Hpcl")
-        as (pc1 pc2 pt) "(Hpl'' & Hpl' & Hpc1 & Hpc2)".
+    - iDestruct "H" as (vr' vsr' m' pl'' ->) "(Hle & Hml' & H) /=".
+      iDestruct (iProto_le_send_inv with "Hle") as (a ml') "[>Hm Hle]".
+      iDestruct (iProto_message_equivI with "Hm") as (<-) "Hm".
+      iSpecialize ("Hle" with "[Hml' Hm] Hml").
+      { by iRewrite ("Hm" $! vr' (Next pl'')) in "Hml'". }
+      iMod "Hle" as (m1 m2 pt) "(Hpl'' & Hpl' & Hm1 & Hm2)". iIntros "!>".
       iDestruct (iProto_interp_le_l with "H Hpl''") as "H".
-      iDestruct ("IH" with "[%] [//] H Hpc1") as "H"; [simpl; lia|..].
+      iDestruct ("IH" with "[%] [//] H Hm1") as "H"; [simpl; lia|..].
       iNext. iApply iProto_interp_unfold. iRight; iRight.
       iExists vr', vsr', _, pt. iSplit; [done|]. by iFrame.
   Qed.
 
-  Lemma iProto_interp_recv vl vsl vsr pl pr pcr :
+  Lemma iProto_interp_recv vl vsl vsr pl pr mr :
     iProto_interp (vl :: vsl) vsr pl pr -∗
-    iProto_le pr (proto_message Recv pcr) -∗
-    ▷ ∃ pr, pcr vl pr ∗ iProto_interp vsl vsr pl pr.
+    pr ⊑ (<?> mr) -∗
+    ◇ ∃ pr, mr vl (Next pr) ∗ ▷ iProto_interp vsl vsr pl pr.
   Proof.
     iIntros "H Hle". iDestruct (iProto_interp_le_r with "H Hle") as "H".
     clear pr. remember (length vsr) as n eqn:Hn.
     iInduction (lt_wf n) as [n _] "IH" forall (vsr pl Hn); subst.
     rewrite !iProto_interp_unfold. iDestruct "H" as "[H|[H|H]]".
     - iClear "IH". iDestruct "H" as (p [=]) "_".
-    - iClear "IH". iDestruct "H" as (vl' vsl' pc' pr' [= -> ->]) "(Hpr & Hpc' & Hinterp)".
-      iDestruct (iProto_le_recv_inv with "Hpr") as (pc'') "[Hpc Hpr]".
-      iDestruct (proto_message_equivI with "Hpc") as (_) "{Hpc} #Hpc".
-      iIntros "!>".
-      iDestruct ("Hpr" $! vl' pr' with "[Hpc']") as (pr'') "[Hler Hpr]".
-      { by iRewrite -("Hpc" $! vl' pr'). }
-      iExists pr''. iFrame "Hpr".
-      by iApply (iProto_interp_le_r with "Hinterp").
-    - iDestruct "H" as (vr vsr' pc' pl'' ->) "(Hpl & Hpc' & Hinterp)".
-      iDestruct ("IH" with "[%] [//] Hinterp") as (pr) "[Hpc Hinterp]"; [simpl; lia|].
-      iIntros "!>". iExists pr. iFrame "Hpc".
+    - iClear "IH". iDestruct "H" as (vl' vsl' m' pr' [= -> ->]) "(Hpr & Hm' & H)".
+      iDestruct (iProto_le_recv_inv with "Hpr") as (m'') "[>Hm Hpr]".
+      iDestruct (iProto_message_equivI with "Hm") as (_) "{Hm} #Hm".
+      iMod ("Hpr" $! vl' pr' with "[Hm']") as (pr'') "[Hler Hpr]".
+      { by iRewrite -("Hm" $! vl' (Next pr')). }
+      iIntros "!>". iExists pr''. iFrame "Hpr".
+      by iApply (iProto_interp_le_r with "H").
+    - iDestruct "H" as (vr vsr' m' pl'' ->) "(Hpl & Hm' & H)".
+      iMod ("IH" with "[%] [//] H") as (pr) "[Hm H]"; [simpl; lia|].
+      iIntros "!>". iExists pr. iFrame "Hm".
       iApply iProto_interp_unfold. iRight; iRight. eauto 20 with iFrame.
   Qed.
 
@@ -963,7 +1076,7 @@ Section proto.
   Proof. apply (ne_proper _). Qed.
 
   Lemma iProto_own_le γ s p1 p2 :
-    iProto_own γ s p1 -∗ ▷ iProto_le p1 p2 -∗ iProto_own γ s p2.
+    iProto_own γ s p1 -∗ ▷ (p1 ⊑ p2) -∗ iProto_own γ s p2.
   Proof.
     iDestruct 1 as (p1') "[Hle H]". iIntros "Hle'".
     iExists p1'. iFrame "H". by iApply (iProto_le_trans with "Hle").
@@ -985,91 +1098,157 @@ Section proto.
     iSplitL "H◯l"; iExists _; iFrame; iApply iProto_le_refl.
   Qed.
 
-  Lemma iProto_send_l {TT} γ (pc : TT → V * iProp Σ * iProto Σ V) (x : TT) vsr vsl :
+  Lemma iProto_send_l γ m vsr vsl vl p :
     iProto_ctx γ vsl vsr -∗
-    iProto_own γ Left (iProto_message Send pc) -∗
-    (pc x).1.2 ==∗
-      ▷^(length vsr) iProto_ctx γ (vsl ++ [(pc x).1.1]) vsr ∗
-      iProto_own γ Left (pc x).2.
+    iProto_own γ Left (<!> m) -∗
+    m vl (Next p) ==∗
+      ▷^(length vsr) iProto_ctx γ (vsl ++ [vl]) vsr ∗
+      iProto_own γ Left p.
   Proof.
-    rewrite iProto_message_eq. iDestruct 1 as (pl pr) "(H●l & H●r & Hinterp)".
-    iDestruct 1 as (p) "[Hle H◯]". iIntros "Hpc".
+    iDestruct 1 as (pl pr) "(H●l & H●r & Hinterp)".
+    iDestruct 1 as (pl') "[Hle H◯]". iIntros "Hm".
     iDestruct (iProto_own_auth_agree with "H●l H◯") as "#Hp".
-    iAssert (▷ iProto_le pl (iProto_message_def Send pc))%I
+    iAssert (▷ (pl ⊑ <!> m))%I
       with "[Hle]" as "{Hp} Hle"; first (iNext; by iRewrite "Hp").
-    iDestruct (iProto_interp_send ((pc x).1.1) with "Hinterp Hle [Hpc]") as "Hinterp".
+    iDestruct (iProto_interp_send with "Hinterp Hle [Hm]") as "Hinterp".
     { simpl. auto. }
-    iMod (iProto_own_auth_update _ _ _ _ (pc x).2 with "H●l H◯") as "[H●l H◯]".
+    iMod (iProto_own_auth_update _ _ _ _ p with "H●l H◯") as "[H●l H◯]".
     iIntros "!>". iSplitR "H◯".
-    - iIntros "!>". iExists (pc x).2, pr. iFrame.
-    - iExists (pc x).2. iFrame. iApply iProto_le_refl.
+    - iIntros "!>". iExists p, pr. iFrame.
+    - iExists p. iFrame. iApply iProto_le_refl.
   Qed.
 
-  Lemma iProto_send_r {TT} γ (pc : TT → V * iProp Σ * iProto Σ V) (x : TT) vsr vsl :
+  Lemma iProto_send_r γ m vsr vsl vr p :
     iProto_ctx γ vsl vsr -∗
-    iProto_own γ Right (iProto_message Send pc) -∗
-    (pc x).1.2 ==∗
-      ▷^(length vsl) iProto_ctx γ vsl (vsr ++ [(pc x).1.1]) ∗
-      iProto_own γ Right (pc x).2.
+    iProto_own γ Right (<!> m) -∗
+    m vr (Next p) ==∗
+      ▷^(length vsl) iProto_ctx γ vsl (vsr ++ [vr]) ∗
+      iProto_own γ Right p.
   Proof.
-    rewrite iProto_message_eq. iDestruct 1 as (pl pr) "(H●l & H●r & Hinterp)".
-    iDestruct 1 as (p) "[Hle H◯]". iIntros "Hpc".
+    iDestruct 1 as (pl pr) "(H●l & H●r & Hinterp)".
+    iDestruct 1 as (pr') "[Hle H◯]". iIntros "Hm".
     iDestruct (iProto_own_auth_agree with "H●r H◯") as "#Hp".
-    iAssert (▷ iProto_le pr (iProto_message_def Send pc))%I
+    iAssert (▷ (pr ⊑ <!> m))%I
       with "[Hle]" as "{Hp} Hle"; first (iNext; by iRewrite "Hp").
     iDestruct (iProto_interp_flip with "Hinterp") as "Hinterp".
-    iDestruct (iProto_interp_send ((pc x).1.1) with "Hinterp Hle [Hpc]") as "Hinterp".
+    iDestruct (iProto_interp_send with "Hinterp Hle [Hm]") as "Hinterp".
     { simpl. auto. }
-    iMod (iProto_own_auth_update _ _ _ _ (pc x).2 with "H●r H◯") as "[H●r H◯]".
+    iMod (iProto_own_auth_update _ _ _ _ p with "H●r H◯") as "[H●r H◯]".
     iIntros "!>". iSplitR "H◯".
-    - iIntros "!>". iExists pl, (pc x).2. iFrame. by iApply iProto_interp_flip.
-    - iExists (pc x).2. iFrame. iApply iProto_le_refl.
+    - iIntros "!>". iExists pl, p. iFrame. by iApply iProto_interp_flip.
+    - iExists p. iFrame. iApply iProto_le_refl.
   Qed.
 
-  Lemma iProto_recv_l {TT} γ (pc : TT → V * iProp Σ * iProto Σ V) vr vsr vsl :
+  Lemma iProto_recv_l γ m vr vsr vsl :
     iProto_ctx γ vsl (vr :: vsr) -∗
-    iProto_own γ Left (iProto_message Recv pc) ==∗
-    ▷ ◇ ∃ (x : TT),
-      ⌜ vr = (pc x).1.1 ⌝ ∗
+    iProto_own γ Left (<?> m) ==∗
+    ▷ ◇ ∃ p,
       iProto_ctx γ vsl vsr ∗
-      iProto_own γ Left (pc x).2 ∗
-      ▷ (pc x).1.2.
+      iProto_own γ Left p ∗
+      m vr (Next p).
   Proof.
-    rewrite iProto_message_eq. iDestruct 1 as (pl pr) "(H●l & H●r & Hinterp)".
+    iDestruct 1 as (pl pr) "(H●l & H●r & Hinterp)".
     iDestruct 1 as (p) "[Hle H◯]".
     iDestruct (iProto_own_auth_agree with "H●l H◯") as "#Hp".
     iDestruct (iProto_interp_flip with "Hinterp") as "Hinterp".
-    iDestruct (iProto_interp_recv with "Hinterp [Hle]") as (q) "[Hpc Hinterp]".
+    iDestruct (iProto_interp_recv with "Hinterp [Hle]") as (q) "[Hm Hinterp]".
     { iNext. by iRewrite "Hp". }
     iMod (iProto_own_auth_update _ _ _ _ q with "H●l H◯") as "[H●l H◯]".
-    iIntros "!> !> /=".
-    iMod (bi.later_exist_except_0 with "Hpc") as (x) "(>-> & Hpc & #Hq)".
-    iIntros "!>". iExists x. iSplit; [done|]. iFrame "Hpc". iSplitR "H◯".
+    iIntros "!> !> /=". iMod "Hm"; iMod "Hinterp". iIntros "!>".
+    iExists q. iFrame "Hm". iSplitR "H◯".
     - iExists q, pr. iFrame. by iApply iProto_interp_flip.
-    - iExists q. iIntros "{$H◯} !>". iRewrite "Hq". iApply iProto_le_refl.
+    - iExists q. iIntros "{$H◯} !>". iApply iProto_le_refl.
   Qed.
 
-  Lemma iProto_recv_r {TT} γ (pc : TT → V * iProp Σ * iProto Σ V) vl vsr vsl :
+  Lemma iProto_recv_r γ m vl vsr vsl :
     iProto_ctx γ (vl :: vsl) vsr -∗
-    iProto_own γ Right (iProto_message Recv pc) ==∗
-    ▷ ◇ ∃ (x : TT),
-      ⌜ vl = (pc x).1.1 ⌝ ∗
+    iProto_own γ Right (<?> m) ==∗
+    ▷ ◇ ∃ p,
       iProto_ctx γ vsl vsr ∗
-      iProto_own γ Right (pc x).2 ∗
-      ▷ (pc x).1.2.
+      iProto_own γ Right p ∗
+      m vl (Next p).
   Proof.
-    rewrite iProto_message_eq. iDestruct 1 as (pl pr) "(H●l & H●r & Hinterp)".
+    iDestruct 1 as (pl pr) "(H●l & H●r & Hinterp)".
     iDestruct 1 as (p) "[Hle H◯]".
     iDestruct (iProto_own_auth_agree with "H●r H◯") as "#Hp".
-    iDestruct (iProto_interp_recv with "Hinterp [Hle]") as (q) "[Hpc Hinterp]".
+    iDestruct (iProto_interp_recv with "Hinterp [Hle]") as (q) "[Hm Hinterp]".
     { iNext. by iRewrite "Hp". }
     iMod (iProto_own_auth_update _ _ _ _ q with "H●r H◯") as "[H●r H◯]".
-    iIntros "!> !> /=".
-    iMod (bi.later_exist_except_0 with "Hpc") as (x) "(>-> & Hpc & #Hq)".
-    iIntros "!>". iExists x. iSplit; [done|]. iFrame "Hpc". iSplitR "H◯".
+    iIntros "!> !> /=". iMod "Hm"; iMod "Hinterp". iIntros "!>".
+    iExists q. iFrame "Hm". iSplitR "H◯".
     - iExists pl, q. iFrame.
-    - iExists q. iIntros "{$H◯} !>". iRewrite "Hq". iApply iProto_le_refl.
+    - iExists q. iIntros "{$H◯} !>". iApply iProto_le_refl.
   Qed.
+
+  (** The instances below make it possible to use the tactics [iIntros],
+  [iExist], [iSplitL]/[iSplitR], [iFrame] and [iModIntro] on [iProto_le] goals. *)
+  Global Instance iProto_le_from_forall_l {A} a (m1 : A → iMsg Σ V) m2 :
+    FromForall ((<? x> m1 x) ⊑ (<a> m2)) (λ x, (<?> m1 x) ⊑ (<a> m2))%I | 10.
+  Proof. apply iProto_le_exist_elim_l. Qed.
+  Global Instance iProto_le_from_forall_r {A} a m1 (m2 : A → iMsg Σ V) :
+    FromForall ((<a> m1) ⊑ (<! x> m2 x)) (λ x, (<a> m1) ⊑ (<!> m2 x))%I | 11.
+  Proof. apply iProto_le_exist_elim_r. Qed.
+
+  Global Instance iProto_le_from_wand_l a m v P p :
+    TCIf (TCEq P True%I) False TCTrue →
+    FromWand ((<?> MSG v {{ P }}; p) ⊑ (<a> m)) P ((<?> MSG v; p) ⊑ (<a> m)) | 10.
+  Proof. intros _. apply iProto_le_payload_elim_l. Qed.
+  Global Instance iProto_le_from_wand_r a m v P p :
+    FromWand ((<a> m) ⊑ (<!> MSG v {{ P }}; p)) P ((<a> m) ⊑ (<!> MSG v; p)) | 11.
+  Proof. apply iProto_le_payload_elim_r. Qed.
+
+  Global Instance iProto_le_from_exist_l {A} (m : A → iMsg Σ V) p :
+    FromExist ((<! x> m x) ⊑ p) (λ a, (<!> m a) ⊑ p)%I | 10.
+  Proof.
+    rewrite /FromExist. iDestruct 1 as (x) "H".
+    iApply (iProto_le_trans with "[] H"). iApply iProto_le_exist_intro_l.
+  Qed.
+  Global Instance iProto_le_from_exist_r {A} (m : A → iMsg Σ V) p :
+    FromExist (p ⊑ <? x> m x) (λ a, p ⊑ (<?> m a))%I | 11.
+  Proof.
+    rewrite /FromExist. iDestruct 1 as (x) "H".
+    iApply (iProto_le_trans with "H"). iApply iProto_le_exist_intro_r.
+  Qed.
+
+  Global Instance iProto_le_from_sep_l m v P p :
+    FromSep ((<!> MSG v {{ P }}; p) ⊑ (<!> m)) P ((<!> MSG v; p) ⊑ (<!> m)) | 10.
+  Proof.
+    rewrite /FromSep. iIntros "[HP H]".
+    iApply (iProto_le_trans with "[HP] H"). by iApply iProto_le_payload_intro_l.
+  Qed.
+  Global Instance iProto_le_from_sep_r m v P p :
+    FromSep ((<?> m) ⊑ (<?> MSG v {{ P }}; p)) P ((<?> m) ⊑ (<?> MSG v; p)) | 11.
+  Proof.
+    rewrite /FromSep. iIntros "[HP H]".
+    iApply (iProto_le_trans with "H"). by iApply iProto_le_payload_intro_r.
+  Qed.
+
+  Global Instance iProto_le_frame_l q m v R P Q p :
+    Frame q R P Q →
+    Frame q R ((<!> MSG v {{ P }}; p) ⊑ (<!> m))
+              ((<!> MSG v {{ Q }}; p) ⊑ (<!> m)) | 10.
+  Proof.
+    rewrite /Frame /=. iIntros (HP) "[HR H]".
+    iApply (iProto_le_trans with "[HR] H"). iApply iProto_le_payload_elim_r.
+    iIntros "HQ". iApply iProto_le_payload_intro_l. iApply HP; iFrame.
+  Qed.
+  Global Instance iProto_le_frame_r q m v R P Q p :
+    Frame q R P Q →
+    Frame q R ((<?> m) ⊑ (<?> MSG v {{ P }}; p))
+              ((<?> m) ⊑ (<?> MSG v {{ Q }}; p)) | 11.
+  Proof.
+    rewrite /Frame /=. iIntros (HP) "[HR H]".
+    iApply (iProto_le_trans with "H"). iApply iProto_le_payload_elim_l.
+    iIntros "HQ". iApply iProto_le_payload_intro_r. iApply HP; iFrame.
+  Qed.
+
+  Global Instance iProto_le_from_modal a v p1 p2 :
+    FromModal (modality_instances.modality_laterN 1) (p1 ⊑ p2)
+              ((<a> MSG v; p1) ⊑ (<a> MSG v; p2)) (p1 ⊑ p2).
+  Proof. apply iProto_le_base. Qed.
 End proto.
 
 Typeclasses Opaque iProto_ctx iProto_own.
+
+Hint Extern 0 (environments.envs_entails _ (?x ⊑ ?y)) =>
+  first [is_evar x; fail 1 | is_evar y; fail 1|iApply iProto_le_refl] : core.
