theories/logrel/subtyping_rules.v
@@ -10,11 +10,7 @@ Section subtyping_rules.
 
   (** Generic rules *)
   Lemma lty_le_refl {k} (M : lty Σ k) : ⊢ M <: M.
-  Proof.
-    destruct k.
-    - by iIntros (v) "!> H".
-    - iModIntro. iApply iProto_le_refl.
-  Qed.
+  Proof. destruct k. by iIntros (v) "!> H". by iModIntro. Qed.
   Lemma lty_le_trans {k} (M1 M2 M3 : lty Σ k) : M1 <: M2 -∗ M2 <: M3 -∗ M1 <: M3.
   Proof.
     destruct k.
@@ -254,143 +250,93 @@ Section subtyping_rules.
     ▷ (A2 <: A1) -∗ ▷ (S1 <: S2) -∗
     (<!!> A1 ; S1) <: (<!!> A2 ; S2).
   Proof.
-    iIntros "#HAle #HSle !>". iApply iProto_le_send; iIntros "!> /=" (x) "H".
-    iDestruct ("HAle" with "H") as "H".
-    eauto with iFrame.
+    iIntros "#HAle #HSle !>" (v) "H". iExists v. 
+    iDestruct ("HAle" with "H") as "$". by iModIntro.
   Qed.
 
   Lemma lty_le_recv A1 A2 S1 S2 :
     ▷ (A1 <: A2) -∗ ▷ (S1 <: S2) -∗
     (<??> A1 ; S1) <: (<??> A2 ; S2).
   Proof.
-    iIntros "#HAle #HSle !>". iApply iProto_le_recv; iIntros "!> /=" (x) "H".
-    iDestruct ("HAle" with "H") as "H".
-    eauto with iFrame.
+    iIntros "#HAle #HSle !>" (v) "H". iExists v.
+    iDestruct ("HAle" with "H") as "$". by iModIntro.
   Qed.
 
   Lemma lty_le_swap_recv_send A1 A2 S :
     ⊢ (<??> A1; <!!> A2; S) <: (<!!> A2; <??> A1; S).
   Proof.
-    iIntros "!>". iApply iProto_le_swap. iIntros "!>" (v1 v2) "/= HS1 HS2".
-    iExists _, _,
-      (tele_app (TT:=[tele _]) (λ v2, (v2, ltty_car A2 v2, lsty_car S))),
-      (tele_app (TT:=[tele _]) (λ v1, (v1, ltty_car A1 v1, lsty_car S))),
-      v2, v1; simpl.
-    do 2 (iSplit; [done|]).
-    iFrame "HS1 HS2".
-    do 2 (iSplitR; [iApply iProto_le_refl|]). by iFrame.
+    iIntros "!>" (v1 v2).
+    iApply iProto_le_trans;
+      [iApply iProto_le_base; iApply (iProto_le_exist_intro_l _ v2)|].
+    iApply iProto_le_trans;
+      [|iApply iProto_le_base; iApply (iProto_le_exist_intro_r _ v1)]; simpl.
+    iApply iProto_le_base_swap.
   Qed.
 
   Lemma lty_le_swap_recv_select A Ss :
-    ⊢ (<??> A; lty_select Ss) <: (lty_select ((λ S, <??> A ; S)%lty <$> Ss)).
+    ⊢ (<??> A; lty_select Ss) <: lty_select ((λ S, <??> A; S) <$> Ss)%lty.
   Proof.
-    iIntros "!>". iApply iProto_le_swap. iIntros "!>" (v1 v2) "/=".
-    iIntros "HS1" (HS2).
-    iExists _, _,
-      (tele_app (TT:=[tele _]) (λ (v2 : Z),(#v2, ⌜is_Some (((λ S : lsty Σ, (<??> A; S)%lty) <$> Ss) !! v2)⌝%I, lsty_car (Ss !!! v2)))),
-      (tele_app (TT:=[tele _]) (λ v1, (v1, ltty_car A v1, lsty_car (Ss !!! v2)))),
-      v2, v1; simpl.
-    do 2 (iSplit; [done|]).
-    iFrame "HS1".
-    iSplitL.
-    - iApply iProto_le_send=> /=.
-      iIntros "!>" (x HSsx). iExists _.
-      rewrite lookup_fmap in HSsx.
-      apply fmap_is_Some in HSsx.
-      do 2 (iSplit; first done).
-      iApply iProto_le_refl.
-    - iSplit; last done.
-      destruct HS2 as [x HS2].
-      rewrite !lookup_total_alt !lookup_fmap /=.
-      rewrite lookup_fmap in HS2.
-      destruct (Ss !! v2); inversion HS2.
-      iApply iProto_le_recv=> /=.
-      iIntros "!>" (y) "H". iExists _.
-      iFrame. iSplit; first done.
-      iApply iProto_le_refl.
+    iIntros "!>" (v1 x2).
+    iApply iProto_le_trans;
+      [iApply iProto_le_base; iApply (iProto_le_exist_intro_l _ x2)|]; simpl.
+    iApply iProto_le_payload_elim_r.
+    rewrite !lookup_total_alt !lookup_fmap fmap_is_Some; iIntros ([S ->]) "/=".
+    iApply iProto_le_trans; [iApply iProto_le_base_swap|]. iSplitL; [by eauto|].
+    iModIntro. by iExists v1.
   Qed.
 
   Lemma lty_le_swap_branch_send A Ss :
-    ⊢ lty_branch ((λ S, <!!> A ; S)%lty <$> Ss) <: (<!!> A ; lty_branch Ss).
+    ⊢ lty_branch ((λ S, <!!> A; S) <$> Ss)%lty <: (<!!> A; lty_branch Ss).
   Proof.
-    iIntros "!>". iApply iProto_le_swap. iIntros "!>" (v1 v2) "/=".
-    iIntros (HS1) "HS2".
-    iExists _, _,
-      (tele_app (TT:=[tele _]) (λ v2, (v2, ltty_car A v2, lsty_car (Ss !!! v1)))),
-      (tele_app (TT:=[tele _]) (λ (v1 : Z),(#v1, ⌜is_Some (((λ S : lsty Σ, (<!!> A; S)%lty) <$> Ss) !! v1)⌝%I, lsty_car (Ss !!! v1)))),
-      v2, v1; simpl.
-    do 2 (iSplit; [done|]).
-    iFrame "HS2".
-    iSplitL.
-    - destruct HS1 as [x HS1].
-      rewrite !lookup_total_alt !lookup_fmap /=.
-      rewrite lookup_fmap in HS1.
-      destruct (Ss !! v1); inversion HS1.
-      iApply iProto_le_send=> /=.
-      iIntros "!>" (y) "H". iExists _.
-      iFrame. iSplit; first done.
-      iApply iProto_le_refl.
-    - iSplit; last done.
-      iApply iProto_le_recv=> /=.
-      iIntros "!>" (y HSsy). iExists _.
-      rewrite lookup_fmap in HSsy.
-      apply fmap_is_Some in HSsy.
-      do 2 (iSplit; first done).
-      iApply iProto_le_refl.
+    iIntros "!>" (x1 v2).
+    iApply iProto_le_trans;
+      [|iApply iProto_le_base; iApply (iProto_le_exist_intro_r _ x1)]; simpl.
+    iApply iProto_le_payload_elim_l.
+    rewrite !lookup_total_alt !lookup_fmap fmap_is_Some; iIntros ([S ->]) "/=".
+    iApply iProto_le_trans; [|iApply iProto_le_base_swap]. iSplitL; [by eauto|].
+    iModIntro. by iExists v2.
   Qed.
 
   Lemma lty_le_select (Ss1 Ss2 : gmap Z (lsty Σ)) :
     ▷ ([∗ map] S1;S2 ∈ Ss1; Ss2, S1 <: S2) -∗
     lty_select Ss1 <: lty_select Ss2.
   Proof.
-    iIntros "#H1 !>". iApply iProto_le_send; iIntros "!>" (x Hsome).
-    iExists x. iSplit; first done. iSplit.
-    - iDestruct (big_sepM2_forall with "H1") as "[% _]".
-      iPureIntro. naive_solver.
-    - iDestruct (big_sepM2_forall with "H1") as "[% H]".
-      iApply ("H" with "[] []").
-      + iPureIntro. apply lookup_lookup_total; naive_solver.
-      + iPureIntro. by apply lookup_lookup_total.
+    iIntros "#H !>" (x); iDestruct 1 as %[S2 HSs2]. iExists x.
+    iDestruct (big_sepM2_forall with "H") as "{H} [>% H]".
+    assert (is_Some (Ss1 !! x)) as [S1 HSs1] by naive_solver.
+    rewrite HSs1. iSplitR; [by eauto|].
+    iIntros "!>". rewrite !lookup_total_alt HSs1 HSs2 /=.
+    by iApply ("H" with "[] []").
   Qed.
   Lemma lty_le_select_subseteq (Ss1 Ss2 : gmap Z (lsty Σ)) :
     Ss2 ⊆ Ss1 →
     ⊢ lty_select Ss1 <: lty_select Ss2.
   Proof.
-    iIntros (Hle) "!>". iApply iProto_le_send; iIntros "!>" (x Hsome).
-    iExists _. iSplit; first done. iSplit.
-    { iPureIntro. by eapply lookup_weaken_is_Some. }
-    destruct Hsome as [P H1].
-    assert (Ss1 !! x = Some P) by eauto using lookup_weaken.
-    rewrite (lookup_total_correct Ss1 x P) //.
-    rewrite (lookup_total_correct Ss2 x P) //.
-    iApply iProto_le_refl.
+    intros; iIntros "!>" (x); iDestruct 1 as %[S HSs2]. iExists x.
+    assert (Ss1 !! x = Some S) as HSs1 by eauto using lookup_weaken.
+    rewrite HSs1. iSplitR; [by eauto|].
+    iIntros "!>". by rewrite !lookup_total_alt HSs1 HSs2 /=.
   Qed.
 
   Lemma lty_le_branch (Ss1 Ss2 : gmap Z (lsty Σ)) :
     ▷ ([∗ map] S1;S2 ∈ Ss1; Ss2, S1 <: S2) -∗
     lty_branch Ss1 <: lty_branch Ss2.
   Proof.
-    iIntros "#H1 !>". iApply iProto_le_recv; iIntros "!>" (x Hsome).
-    iExists x. iSplit; first done. iSplit.
-    - iDestruct (big_sepM2_forall with "H1") as "[% _]".
-      iPureIntro. by naive_solver.
-    - iDestruct (big_sepM2_forall with "H1") as "[% H]".
-      iApply ("H" with "[] []").
-      + iPureIntro. by apply lookup_lookup_total.
-      + iPureIntro. by apply lookup_lookup_total; naive_solver.
+    iIntros "#H !>" (x); iDestruct 1 as %[S1 HSs1]. iExists x.
+    iDestruct (big_sepM2_forall with "H") as "{H} [>% H]".
+    assert (is_Some (Ss2 !! x)) as [S2 HSs2] by naive_solver.
+    rewrite HSs2. iSplitR; [by eauto|].
+    iIntros "!>". rewrite !lookup_total_alt HSs1 HSs2 /=.
+    by iApply ("H" with "[] []").
   Qed.
   Lemma lty_le_branch_subseteq (Ss1 Ss2 : gmap Z (lsty Σ)) :
     Ss1 ⊆ Ss2 →
     ⊢ lty_branch Ss1 <: lty_branch Ss2.
   Proof.
-    iIntros (Hle) "!>". iApply iProto_le_recv; iIntros "!>" (x Hsome).
-    iExists _. iSplit; first done. iSplit.
-    { iPureIntro. by eapply lookup_weaken_is_Some. }
-    destruct Hsome as [P ?].
-    assert (Ss2 !! x = Some P) by eauto using lookup_weaken.
-    rewrite (lookup_total_correct Ss1 x P) //.
-    rewrite (lookup_total_correct Ss2 x P) //.
-    iApply iProto_le_refl.
+    intros; iIntros "!>" (x); iDestruct 1 as %[S HSs1]. iExists x.
+    assert (Ss2 !! x = Some S) as HSs2 by eauto using lookup_weaken.
+    rewrite HSs2. iSplitR; [by eauto|].
+    iIntros "!>". by rewrite !lookup_total_alt HSs1 HSs2 /=.
   Qed.
 
   (** Algebraic laws *)
@@ -400,47 +346,32 @@ Section subtyping_rules.
   Proof. iIntros "#H1 #H2 !>". by iApply iProto_le_app. Qed.
 
   Lemma lty_le_app_id_l S : ⊢ (END <++> S) <:> S.
-  Proof. rewrite /lty_app left_id. iSplit; iModIntro; iApply iProto_le_refl. Qed.
+  Proof. rewrite /lty_app left_id. iSplit; by iModIntro. Qed.
   Lemma lty_le_app_id_r S : ⊢ (S <++> END) <:> S.
-  Proof. rewrite /lty_app right_id. iSplit; iModIntro; iApply iProto_le_refl. Qed.
+  Proof. rewrite /lty_app right_id. iSplit; by iModIntro. Qed.
   Lemma lty_le_app_assoc S1 S2 S3 :
     ⊢ (S1 <++> S2) <++> S3 <:> S1 <++> (S2 <++> S3).
-  Proof. rewrite /lty_app assoc. iSplit; iModIntro; iApply iProto_le_refl. Qed.
+  Proof. rewrite /lty_app assoc. iSplit; by iModIntro. Qed.
 
   Lemma lty_le_app_send A S1 S2 : ⊢ (<!!> A; S1) <++> S2 <:> (<!!> A; S1 <++> S2).
   Proof.
-    rewrite /lty_app iProto_app_message_tele.
-    iSplit; iIntros "!>"; iApply iProto_le_refl.
+    rewrite /lty_app iProto_app_message iMsg_app_exist.
+    setoid_rewrite iMsg_app_base. iSplit; by iIntros "!> /=".
   Qed.
   Lemma lty_le_app_recv A S1 S2 : ⊢ (<??> A; S1) <++> S2 <:> (<??> A; S1 <++> S2).
   Proof.
-    rewrite /lty_app iProto_app_message_tele.
-    iSplit; iIntros "!>"; iApply iProto_le_refl.
+    rewrite /lty_app iProto_app_message iMsg_app_exist.
+    setoid_rewrite iMsg_app_base. iSplit; by iIntros "!> /=".
   Qed.
 
   Lemma lty_le_app_choice a (Ss : gmap Z (lsty Σ)) S2 :
     ⊢ lty_choice a Ss <++> S2 <:> lty_choice a ((.<++> S2) <$> Ss)%lty.
   Proof.
-    destruct a.
-    - rewrite /lty_app iProto_app_message_tele. iSplit; iIntros "!> /=".
-      + iApply iProto_le_send; iIntros "!>" (x [S HSs]); simpl in *.
-        move: HSs; rewrite lookup_fmap fmap_Some; intros (S'&HSs&->).
-        iExists _; do 2 (iSplit; [by eauto|]).
-        rewrite !lookup_total_alt lookup_fmap !HSs /=. iApply iProto_le_refl.
-      + iApply iProto_le_send; iIntros "!>" (x [S HSs]); simpl in *.
-        iExists _; iSplit; [by eauto|].
-        rewrite !lookup_total_alt lookup_fmap !HSs /=.
-        iSplit; [by eauto|]. iApply iProto_le_refl.
-    - rewrite /lty_app iProto_app_message_tele. iSplit; iIntros "!> /=".
-      + iApply iProto_le_recv; iIntros "!>" (x [S HSs]); simpl in *.
-        iExists _; iSplit; [by eauto|].
-        rewrite !lookup_total_alt lookup_fmap !HSs /=.
-        iSplit; [by eauto|]. iApply iProto_le_refl.
-      + iApply iProto_le_recv; iIntros "!>" (x [S HSs]); simpl in *.
-        move: HSs; rewrite lookup_fmap fmap_Some; intros (S'&HSs&->).
-        iExists _; iSplit; [by eauto|].
-        rewrite !lookup_total_alt lookup_fmap !HSs /=.
-        iSplit; [by eauto|]. iApply iProto_le_refl.
+    rewrite /lty_app /lty_choice iProto_app_message iMsg_app_exist;
+      setoid_rewrite iMsg_app_base; setoid_rewrite lookup_total_alt;
+      setoid_rewrite lookup_fmap; setoid_rewrite fmap_is_Some.
+    iSplit; iIntros "!> /="; destruct a; iIntros (x); iExists x;
+      iDestruct 1 as %[S ->]; iSplitR; eauto.
   Qed.
   Lemma lty_le_app_select A Ss S2 :
     ⊢ lty_select Ss <++> S2 <:> lty_select ((.<++> S2) <$> Ss)%lty.
@@ -462,8 +393,8 @@ Section subtyping_rules.
   Lemma lty_le_dual_message a A S :
     ⊢ lty_dual (lty_message a A S) <:> lty_message (action_dual a) A (lty_dual S).
   Proof.
-    iSplit; iIntros "!>"; rewrite /lty_dual iProto_dual_message_tele;
-      iApply iProto_le_refl.
+    rewrite /lty_dual iProto_dual_message iMsg_dual_exist.
+    setoid_rewrite iMsg_dual_base. iSplit; by iIntros "!> /=".
   Qed.
   Lemma lty_le_dual_send A S : ⊢ lty_dual (<!!> A; S) <:> (<??> A; lty_dual S).
   Proof. apply lty_le_dual_message. Qed.
@@ -473,26 +404,11 @@ Section subtyping_rules.
   Lemma lty_le_dual_choice a (Ss : gmap Z (lsty Σ)) :
     ⊢ lty_dual (lty_choice a Ss) <:> lty_choice (action_dual a) (lty_dual <$> Ss).
   Proof.
-    destruct a.
-    - rewrite /lty_dual iProto_dual_message_tele. iSplit; iIntros "!> /=".
-      + iApply iProto_le_recv; iIntros "!>" (x [S HSs]); simpl in *.
-        iExists _; iSplit; [by eauto|].
-        rewrite !lookup_total_alt lookup_fmap !HSs /=.
-        iSplit; [by eauto|]. iApply iProto_le_refl.
-      + iApply iProto_le_recv; iIntros "!>" (x [S HSs]); simpl in *.
-        move: HSs; rewrite lookup_fmap fmap_Some; intros (S'&HSs&->).
-        iExists _; iSplit; [by eauto|].
-        rewrite !lookup_total_alt lookup_fmap !HSs /=.
-        iSplit; [by eauto|]. iApply iProto_le_refl.
-    - rewrite /lty_dual iProto_dual_message_tele. iSplit; iIntros "!> /=".
-      + iApply iProto_le_send; iIntros "!>" (x [S HSs]); simpl in *.
-        move: HSs; rewrite lookup_fmap fmap_Some; intros (S'&HSs&->).
-        iExists _; do 2 (iSplit; [by eauto|]).
-        rewrite !lookup_total_alt lookup_fmap !HSs /=. iApply iProto_le_refl.
-      + iApply iProto_le_send; iIntros "!>" (x [S HSs]); simpl in *.
-        iExists _; iSplit; [by eauto|].
-        rewrite !lookup_total_alt lookup_fmap !HSs /=.
-        iSplit; [by eauto|]. iApply iProto_le_refl.
+    rewrite /lty_dual /lty_choice iProto_dual_message iMsg_dual_exist;
+      setoid_rewrite iMsg_dual_base; setoid_rewrite lookup_total_alt;
+      setoid_rewrite lookup_fmap; setoid_rewrite fmap_is_Some.
+    iSplit; iIntros "!> /="; destruct a; iIntros (x); iExists x;
+      iDestruct 1 as %[S ->]; iSplitR; eauto.
   Qed.
 
   Lemma lty_le_dual_select (Ss : gmap Z (lsty Σ)) :
